Refactor in progress
Signed-off-by: zeramorphic <zeramorphic@proton.me>

src/phase2/fill_atom_orbits.lean
@@ -1,4 +1,4 @@
-import phase2.weak_approx
+import phase2.near_litter_action
 
 open cardinal quiver set sum with_bot
 open_locale cardinal classical pointwise
@@ -12,30 +12,30 @@ variables [params.{u}]
 # Filling in orbits of atoms
 -/
 
-namespace weak_near_litter_approx
+namespace near_litter_action
 
-variables (w : weak_near_litter_approx)
+variables (φ : near_litter_action) (hφ : φ.lawful)
 
-def need_forward_images : set atom := w.atom_map.ran \ w.atom_map.dom
-def need_backward_images : set atom := w.atom_map.dom \ w.atom_map.ran
+def need_forward_images : set atom := φ.atom_map.ran \ φ.atom_map.dom
+def need_backward_images : set atom := φ.atom_map.dom \ φ.atom_map.ran
 
-lemma atom_map_ran_small : small w.atom_map.ran :=
+lemma atom_map_ran_small : small φ.atom_map.ran :=
 begin
-  have : small (w.atom_map_or_else '' w.atom_map.dom) := small.image w.atom_map_dom_small,
+  have : small (φ.atom_map_or_else '' φ.atom_map.dom) := small.image φ.atom_map_dom_small,
   refine small.mono _ this,
   rintros _ ⟨a, ha, rfl⟩,
   refine ⟨a, ha, _⟩,
   rw atom_map_or_else_of_dom,
 end
 
-lemma need_forward_images_small : small w.need_forward_images :=
-small.mono (diff_subset _ _) w.atom_map_ran_small
+lemma need_forward_images_small : small φ.need_forward_images :=
+small.mono (diff_subset _ _) φ.atom_map_ran_small
 
-lemma need_backward_images_small : small w.need_backward_images :=
-small.mono (diff_subset _ _) w.atom_map_dom_small
+lemma need_backward_images_small : small φ.need_backward_images :=
+small.mono (diff_subset _ _) φ.atom_map_dom_small
 
 lemma mk_diff_dom_ran (L : litter) :
-  #(litter_set L \ (w.atom_map.dom ∪ w.atom_map.ran) : set atom) = #κ :=
+  #(litter_set L \ (φ.atom_map.dom ∪ φ.atom_map.ran) : set atom) = #κ :=
 begin
   refine le_antisymm _ _,
   { refine ⟨⟨λ a, a.1.2, _⟩⟩,
@@ -45,120 +45,120 @@ begin
     exact h, },
   { by_contra' h,
     have := add_lt_of_lt κ_regular.aleph_0_le h
-      (small.union w.atom_map_dom_small w.atom_map_ran_small),
+      (small.union φ.atom_map_dom_small φ.atom_map_ran_small),
     have := (le_mk_diff_add_mk (litter_set L) _).trans_lt this,
     simp only [mk_litter_set, lt_self_iff_false] at this,
     exact this, },
 end
 
 lemma need_images_small (L : litter) :
-  #(ℕ × w.need_backward_images ⊕ ℕ × w.need_forward_images) < #κ :=
+  #(ℕ × φ.need_backward_images ⊕ ℕ × φ.need_forward_images) < #κ :=
 begin
   simp only [mk_prod, mk_denumerable, lift_aleph_0, lift_uzero, mk_diff_dom_ran, mk_sum, lift_id],
   rw ← mul_add,
   refine lt_of_le_of_lt (mul_le_max _ _) (max_lt (max_lt _ _) _),
   exact Λ_limit.aleph_0_le.trans_lt Λ_lt_κ,
-  exact add_lt_of_lt κ_regular.aleph_0_le w.need_backward_images_small w.need_forward_images_small,
+  exact add_lt_of_lt κ_regular.aleph_0_le φ.need_backward_images_small φ.need_forward_images_small,
   exact Λ_limit.aleph_0_le.trans_lt Λ_lt_κ,
 end
 
 lemma le_mk_diff_dom_ran (L : litter) :
-  #(ℕ × w.need_backward_images ⊕ ℕ × w.need_forward_images) ≤
-    #(litter_set L \ (w.atom_map.dom ∪ w.atom_map.ran) : set atom) :=
+  #(ℕ × φ.need_backward_images ⊕ ℕ × φ.need_forward_images) ≤
+    #(litter_set L \ (φ.atom_map.dom ∪ φ.atom_map.ran) : set atom) :=
 begin
   rw [mk_diff_dom_ran],
-  exact (w.need_images_small L).le,
+  exact (φ.need_images_small L).le,
 end
 
 def orbit_set (L : litter) : set atom :=
-(le_mk_iff_exists_subset.mp (w.le_mk_diff_dom_ran L)).some
+(le_mk_iff_exists_subset.mp (φ.le_mk_diff_dom_ran L)).some
 
 lemma orbit_set_subset (L : litter) :
-  w.orbit_set L ⊆ litter_set L \ (w.atom_map.dom ∪ w.atom_map.ran) :=
-(le_mk_iff_exists_subset.mp (w.le_mk_diff_dom_ran L)).some_spec.1
+  φ.orbit_set L ⊆ litter_set L \ (φ.atom_map.dom ∪ φ.atom_map.ran) :=
+(le_mk_iff_exists_subset.mp (φ.le_mk_diff_dom_ran L)).some_spec.1
 
 lemma not_mem_need_forward_images_of_mem_orbit_set {a : atom} {L : litter}
-  (h : a ∈ w.orbit_set L) : a ∉ w.need_forward_images :=
-λ ha, (w.orbit_set_subset L h).2 (or.inr ha.1)
+  (h : a ∈ φ.orbit_set L) : a ∉ φ.need_forward_images :=
+λ ha, (φ.orbit_set_subset L h).2 (or.inr ha.1)
 
 lemma not_mem_need_backward_images_of_mem_orbit_set {a : atom} {L : litter}
-  (h : a ∈ w.orbit_set L) : a ∉ w.need_backward_images :=
-λ ha, (w.orbit_set_subset L h).2 (or.inl ha.1)
+  (h : a ∈ φ.orbit_set L) : a ∉ φ.need_backward_images :=
+λ ha, (φ.orbit_set_subset L h).2 (or.inl ha.1)
 
 lemma mk_orbit_set (L : litter) :
-  #(w.orbit_set L) = #(ℕ × w.need_backward_images ⊕ ℕ × w.need_forward_images) :=
-(le_mk_iff_exists_subset.mp (w.le_mk_diff_dom_ran L)).some_spec.2
+  #(φ.orbit_set L) = #(ℕ × φ.need_backward_images ⊕ ℕ × φ.need_forward_images) :=
+(le_mk_iff_exists_subset.mp (φ.le_mk_diff_dom_ran L)).some_spec.2
 
 @[irreducible] noncomputable def orbit_set_equiv (L : litter) :
-  w.orbit_set L ≃ ℕ × w.need_backward_images ⊕ ℕ × w.need_forward_images :=
-(cardinal.eq.mp (w.mk_orbit_set L)).some
+  φ.orbit_set L ≃ ℕ × φ.need_backward_images ⊕ ℕ × φ.need_forward_images :=
+(cardinal.eq.mp (φ.mk_orbit_set L)).some
 
-lemma orbit_set_equiv_injective {a₁ a₂ : ℕ × w.need_backward_images ⊕ ℕ × w.need_forward_images}
-  {L₁ L₂ : litter} (h : ((w.orbit_set_equiv L₁).symm a₁ : atom) = (w.orbit_set_equiv L₂).symm a₂) :
+lemma orbit_set_equiv_injective {a₁ a₂ : ℕ × φ.need_backward_images ⊕ ℕ × φ.need_forward_images}
+  {L₁ L₂ : litter} (h : ((φ.orbit_set_equiv L₁).symm a₁ : atom) = (φ.orbit_set_equiv L₂).symm a₂) :
   L₁ = L₂ ∧ a₁ = a₂ :=
 begin
-  have h₁ := w.orbit_set_subset L₁ ((w.orbit_set_equiv L₁).symm a₁).prop,
-  have h₂ := w.orbit_set_subset L₂ ((w.orbit_set_equiv L₂).symm a₂).prop,
+  have h₁ := φ.orbit_set_subset L₁ ((φ.orbit_set_equiv L₁).symm a₁).prop,
+  have h₂ := φ.orbit_set_subset L₂ ((φ.orbit_set_equiv L₂).symm a₂).prop,
   rw h at h₁,
   cases eq_of_mem_litter_set_of_mem_litter_set h₁.1 h₂.1,
   simp only [subtype.coe_inj, embedding_like.apply_eq_iff_eq] at h,
   exact ⟨rfl, h⟩,
 end
 
-lemma orbit_set_equiv_congr {L L' : litter} {a : atom} (ha : a ∈ w.orbit_set L) (h : L = L') :
-  w.orbit_set_equiv L ⟨a, ha⟩ = w.orbit_set_equiv L' ⟨a, h ▸ ha⟩ :=
+lemma orbit_set_equiv_congr {L L' : litter} {a : atom} (ha : a ∈ φ.orbit_set L) (h : L = L') :
+  φ.orbit_set_equiv L ⟨a, ha⟩ = φ.orbit_set_equiv L' ⟨a, h ▸ ha⟩ :=
 by cases h; refl
 
 lemma orbit_set_equiv_symm_congr {L L' : litter}
-  {a : ℕ × ↥(w.need_backward_images) ⊕ ℕ × ↥(w.need_forward_images)} (h : L = L') :
-  ((w.orbit_set_equiv L).symm a : atom) = (w.orbit_set_equiv L').symm a :=
+  {a : ℕ × ↥(φ.need_backward_images) ⊕ ℕ × ↥(φ.need_forward_images)} (h : L = L') :
+  ((φ.orbit_set_equiv L).symm a : atom) = (φ.orbit_set_equiv L').symm a :=
 by cases h; refl
 
-lemma orbit_set_small (L : litter) : small (w.orbit_set L) :=
+lemma orbit_set_small (L : litter) : small (φ.orbit_set L) :=
 begin
   rw [small, mk_orbit_set],
-  exact w.need_images_small L,
+  exact φ.need_images_small L,
 end
 
-noncomputable def next_forward_image (L : litter) (a : ℕ × w.need_forward_images) : atom :=
-(w.orbit_set_equiv (w.litter_perm L)).symm (inr (a.1 + 1, a.2))
+noncomputable def next_forward_image (L : litter) (a : ℕ × φ.need_forward_images) : atom :=
+(φ.orbit_set_equiv (φ.litter_perm hφ L)).symm (inr (a.1 + 1, a.2))
 
-noncomputable def next_backward_image (L : litter) : ℕ × w.need_backward_images → atom
+noncomputable def next_backward_image (L : litter) : ℕ × φ.need_backward_images → atom
 | (0, a) := a
-| (n + 1, a) := (w.orbit_set_equiv (w.litter_perm L)).symm (inl (n, a))
+| (n + 1, a) := (φ.orbit_set_equiv (φ.litter_perm hφ L)).symm (inl (n, a))
 
-def next_forward_image_domain (L : litter) : set (ℕ × w.need_forward_images) :=
-{a | (a.2 : atom).1 ∈ w.litter_perm.domain ∧ (w.litter_perm^[a.1 + 1] (a.2 : atom).1 = L)}
+def next_forward_image_domain (L : litter) : set (ℕ × φ.need_forward_images) :=
+{a | (a.2 : atom).1 ∈ (φ.litter_perm hφ).domain ∧ ((φ.litter_perm hφ)^[a.1 + 1] (a.2 : atom).1 = L)}
 
-def next_backward_image_domain (L : litter) : set (ℕ × w.need_backward_images) :=
-{a | (a.2 : atom).1 ∈ w.litter_perm.domain ∧ (w.litter_perm.symm^[a.1 + 1] (a.2 : atom).1 = L)}
+def next_backward_image_domain (L : litter) : set (ℕ × φ.need_backward_images) :=
+{a | (a.2 : atom).1 ∈ (φ.litter_perm hφ).domain ∧ ((φ.litter_perm hφ).symm^[a.1 + 1] (a.2 : atom).1 = L)}
 
-lemma mk_mem_next_forward_image_domain (L : litter) (n : ℕ) (a : w.need_forward_images) :
-  (n, a) ∈ w.next_forward_image_domain L ↔
-    (a : atom).1 ∈ w.litter_perm.domain ∧ (w.litter_perm^[n + 1] (a : atom).1 = L) := iff.rfl
+lemma mk_mem_next_forward_image_domain (L : litter) (n : ℕ) (a : φ.need_forward_images) :
+  (n, a) ∈ φ.next_forward_image_domain hφ L ↔
+    (a : atom).1 ∈ (φ.litter_perm hφ).domain ∧ ((φ.litter_perm hφ)^[n + 1] (a : atom).1 = L) := iff.rfl
 
-lemma mk_mem_next_backward_image_domain (L : litter) (n : ℕ) (a : w.need_backward_images) :
-  (n, a) ∈ w.next_backward_image_domain L ↔
-    (a : atom).1 ∈ w.litter_perm.domain ∧ (w.litter_perm.symm^[n + 1] (a : atom).1 = L) := iff.rfl
+lemma mk_mem_next_backward_image_domain (L : litter) (n : ℕ) (a : φ.need_backward_images) :
+  (n, a) ∈ φ.next_backward_image_domain hφ L ↔
+    (a : atom).1 ∈ (φ.litter_perm hφ).domain ∧ ((φ.litter_perm hφ).symm^[n + 1] (a : atom).1 = L) := iff.rfl
 
-lemma next_forward_image_eq {L₁ L₂ : litter} {a b : ℕ × w.need_forward_images}
-  (hL₁ : L₁ ∈ w.litter_perm.domain) (hL₂ : L₂ ∈ w.litter_perm.domain)
-  (h : w.next_forward_image L₁ a = w.next_forward_image L₂ b) : L₁ = L₂ :=
+lemma next_forward_image_eq {L₁ L₂ : litter} {a b : ℕ × φ.need_forward_images}
+  (hL₁ : L₁ ∈ (φ.litter_perm hφ).domain) (hL₂ : L₂ ∈ (φ.litter_perm hφ).domain)
+  (h : φ.next_forward_image hφ L₁ a = φ.next_forward_image hφ L₂ b) : L₁ = L₂ :=
 begin
   rw [next_forward_image, next_forward_image] at h,
-  have ha := w.orbit_set_subset _
-    ((w.orbit_set_equiv (w.litter_perm L₁)).symm (inr (a.1 + 1, a.2))).prop,
-  have hb := w.orbit_set_subset _
-    ((w.orbit_set_equiv (w.litter_perm L₂)).symm (inr (b.1 + 1, b.2))).prop,
+  have ha := φ.orbit_set_subset _
+    ((φ.orbit_set_equiv (φ.litter_perm hφ L₁)).symm (inr (a.1 + 1, a.2))).prop,
+  have hb := φ.orbit_set_subset _
+    ((φ.orbit_set_equiv (φ.litter_perm hφ L₂)).symm (inr (b.1 + 1, b.2))).prop,
   rw h at ha,
-  refine w.litter_perm.inj_on hL₁ hL₂ _,
+  refine (φ.litter_perm hφ).inj_on hL₁ hL₂ _,
   exact eq_of_mem_litter_set_of_mem_litter_set ha.1 hb.1,
 end
 
-lemma next_backward_image_eq {L₁ L₂ : litter} {a b : ℕ × w.need_backward_images}
-  (ha : a ∈ w.next_backward_image_domain L₁) (hb : b ∈ w.next_backward_image_domain L₂)
-  (hL₁ : L₁ ∈ w.litter_perm.domain) (hL₂ : L₂ ∈ w.litter_perm.domain)
-  (h : w.next_backward_image L₁ a = w.next_backward_image L₂ b) : L₁ = L₂ :=
+lemma next_backward_image_eq {L₁ L₂ : litter} {a b : ℕ × φ.need_backward_images}
+  (ha : a ∈ φ.next_backward_image_domain hφ L₁) (hb : b ∈ φ.next_backward_image_domain hφ L₂)
+  (hL₁ : L₁ ∈ (φ.litter_perm hφ).domain) (hL₂ : L₂ ∈ (φ.litter_perm hφ).domain)
+  (h : φ.next_backward_image hφ L₁ a = φ.next_backward_image hφ L₂ b) : L₁ = L₂ :=
 begin
   obtain ⟨m, a⟩ := a,
   obtain ⟨n, b⟩ := b,
@@ -171,31 +171,31 @@ begin
     exact hb.2, },
   { rw subtype.coe_eq_iff at h,
     obtain ⟨h₁, h₂⟩ := h,
-    cases w.not_mem_need_backward_images_of_mem_orbit_set ((w.orbit_set_equiv _).symm _).prop h₁, },
+    cases φ.not_mem_need_backward_images_of_mem_orbit_set ((φ.orbit_set_equiv _).symm _).prop h₁, },
   { symmetry' at h,
     rw subtype.coe_eq_iff at h,
     obtain ⟨h₁, h₂⟩ := h,
-    cases w.not_mem_need_backward_images_of_mem_orbit_set ((w.orbit_set_equiv _).symm _).prop h₁, },
-  { have ha := w.orbit_set_subset _
-      ((w.orbit_set_equiv (w.litter_perm L₁)).symm (inl (m, a))).prop,
-    have hb := w.orbit_set_subset _
-      ((w.orbit_set_equiv (w.litter_perm L₂)).symm (inl (n, b))).prop,
+    cases φ.not_mem_need_backward_images_of_mem_orbit_set ((φ.orbit_set_equiv _).symm _).prop h₁, },
+  { have ha := φ.orbit_set_subset _
+      ((φ.orbit_set_equiv (φ.litter_perm hφ L₁)).symm (inl (m, a))).prop,
+    have hb := φ.orbit_set_subset _
+      ((φ.orbit_set_equiv (φ.litter_perm hφ L₂)).symm (inl (n, b))).prop,
     rw h at ha,
-    refine w.litter_perm.inj_on hL₁ hL₂ _,
+    refine (φ.litter_perm hφ).inj_on hL₁ hL₂ _,
     exact eq_of_mem_litter_set_of_mem_litter_set ha.1 hb.1, },
 end
 
-lemma next_forward_image_injective {L : litter} {a b : ℕ × w.need_forward_images}
-  (h : w.next_forward_image L a = w.next_forward_image L b) : a = b :=
+lemma next_forward_image_injective {L : litter} {a b : ℕ × φ.need_forward_images}
+  (h : φ.next_forward_image hφ L a = φ.next_forward_image hφ L b) : a = b :=
 begin
   simp only [next_forward_image, subtype.coe_inj, embedding_like.apply_eq_iff_eq, prod.mk.inj_iff,
     add_left_inj] at h,
   exact prod.ext h.1 h.2,
 end
 
-lemma next_backward_image_injective {L : litter} {a b : ℕ × w.need_backward_images}
-  (ha : a ∈ w.next_backward_image_domain L) (hb : b ∈ w.next_backward_image_domain L)
-  (h : w.next_backward_image L a = w.next_backward_image L b) : a = b :=
+lemma next_backward_image_injective {L : litter} {a b : ℕ × φ.need_backward_images}
+  (ha : a ∈ φ.next_backward_image_domain hφ L) (hb : b ∈ φ.next_backward_image_domain hφ L)
+  (h : φ.next_backward_image hφ L a = φ.next_backward_image hφ L b) : a = b :=
 begin
   obtain ⟨m, a⟩ := a,
   obtain ⟨n, b⟩ := b,
@@ -207,279 +207,282 @@ begin
   { exact h, },
   { rw subtype.coe_eq_iff at h,
     obtain ⟨h₁, h₂⟩ := h,
-    cases w.not_mem_need_backward_images_of_mem_orbit_set ((w.orbit_set_equiv _).symm _).prop h₁, },
+    cases φ.not_mem_need_backward_images_of_mem_orbit_set ((φ.orbit_set_equiv _).symm _).prop h₁, },
   { symmetry' at h,
     rw subtype.coe_eq_iff at h,
     obtain ⟨h₁, h₂⟩ := h,
-    cases w.not_mem_need_backward_images_of_mem_orbit_set ((w.orbit_set_equiv _).symm _).prop h₁, },
+    cases φ.not_mem_need_backward_images_of_mem_orbit_set ((φ.orbit_set_equiv _).symm _).prop h₁, },
   { exact h, },
 end
 
-lemma next_forward_image_injective' {L₁ L₂ : litter} {a b : ℕ × w.need_forward_images}
-  (hL₁ : L₁ ∈ w.litter_perm.domain) (hL₂ : L₂ ∈ w.litter_perm.domain)
-  (h : w.next_forward_image L₁ a = w.next_forward_image L₂ b) : a = b :=
+lemma next_forward_image_injective' {L₁ L₂ : litter} {a b : ℕ × φ.need_forward_images}
+  (hL₁ : L₁ ∈ (φ.litter_perm hφ).domain) (hL₂ : L₂ ∈ (φ.litter_perm hφ).domain)
+  (h : φ.next_forward_image hφ L₁ a = φ.next_forward_image hφ L₂ b) : a = b :=
 begin
-  cases w.next_forward_image_eq hL₁ hL₂ h,
-  exact w.next_forward_image_injective h,
+  cases φ.next_forward_image_eq hφ hL₁ hL₂ h,
+  exact φ.next_forward_image_injective hφ h,
 end
 
-lemma next_backward_image_injective' {L₁ L₂ : litter} {a b : ℕ × w.need_backward_images}
-  (ha : a ∈ w.next_backward_image_domain L₁) (hb : b ∈ w.next_backward_image_domain L₂)
-  (hL₁ : L₁ ∈ w.litter_perm.domain) (hL₂ : L₂ ∈ w.litter_perm.domain)
-  (h : w.next_backward_image L₁ a = w.next_backward_image L₂ b) : a = b :=
+lemma next_backward_image_injective' {L₁ L₂ : litter} {a b : ℕ × φ.need_backward_images}
+  (ha : a ∈ φ.next_backward_image_domain hφ L₁) (hb : b ∈ φ.next_backward_image_domain hφ L₂)
+  (hL₁ : L₁ ∈ (φ.litter_perm hφ).domain) (hL₂ : L₂ ∈ (φ.litter_perm hφ).domain)
+  (h : φ.next_backward_image hφ L₁ a = φ.next_backward_image hφ L₂ b) : a = b :=
 begin
-  cases w.next_backward_image_eq ha hb hL₁ hL₂ h,
-  exact w.next_backward_image_injective ha hb h,
+  cases φ.next_backward_image_eq hφ ha hb hL₁ hL₂ h,
+  exact φ.next_backward_image_injective hφ ha hb h,
 end
 
 lemma next_forward_image_ne_next_backward_image {L₁ L₂ : litter}
-  {a : ℕ × w.need_forward_images} {b : ℕ × w.need_backward_images} :
-  w.next_forward_image L₁ a ≠ w.next_backward_image L₂ b :=
+  {a : ℕ × φ.need_forward_images} {b : ℕ × φ.need_backward_images} :
+  φ.next_forward_image hφ L₁ a ≠ φ.next_backward_image hφ L₂ b :=
 begin
   obtain ⟨n, b⟩ := b,
   cases n,
   { rw [next_forward_image, next_backward_image],
     refine (ne_of_mem_of_not_mem _
-      (w.orbit_set_subset _ ((w.orbit_set_equiv _).symm _).prop).2).symm,
+      (φ.orbit_set_subset _ ((φ.orbit_set_equiv _).symm _).prop).2).symm,
     exact or.inl b.prop.1, },
   { rw [next_forward_image, next_backward_image],
     intro h,
-    cases (w.orbit_set_equiv_injective h).2, },
+    cases (φ.orbit_set_equiv_injective h).2, },
 end
 
-noncomputable def next_image_core (a : atom) (L : litter) (ha : a ∈ w.orbit_set L) : atom :=
-(w.orbit_set_equiv L ⟨a, ha⟩).elim (w.next_backward_image L) (w.next_forward_image L)
+noncomputable def next_image_core (a : atom) (L : litter) (ha : a ∈ φ.orbit_set L) : atom :=
+(φ.orbit_set_equiv L ⟨a, ha⟩).elim (φ.next_backward_image hφ L) (φ.next_forward_image hφ L)
 
 def next_image_core_domain : set atom :=
-⋃ L ∈ w.litter_perm.domain, coe '' {a : w.orbit_set L | (w.orbit_set_equiv L a).elim
-  (λ b, b ∈ w.next_backward_image_domain L) (λ b, b ∈ w.next_forward_image_domain L)}
+⋃ L ∈ (φ.litter_perm hφ).domain, coe '' {a : φ.orbit_set L | (φ.orbit_set_equiv L a).elim
+  (λ b, b ∈ φ.next_backward_image_domain hφ L) (λ b, b ∈ φ.next_forward_image_domain hφ L)}
 
-lemma next_image_core_domain_small : small w.next_image_core_domain :=
-small.bUnion w.litter_perm_domain_small
-  (λ L hL, small.image (lt_of_le_of_lt (cardinal.mk_subtype_le _) (w.orbit_set_small L)))
+lemma next_image_core_domain_small : small (φ.next_image_core_domain hφ) :=
+small.bUnion (φ.litter_perm_domain_small hφ)
+  (λ L hL, small.image (lt_of_le_of_lt (cardinal.mk_subtype_le _) (φ.orbit_set_small L)))
 
-lemma litter_map_dom_of_mem_next_image_core_domain {a : atom} (h : a ∈ w.next_image_core_domain) :
-  a.1 ∈ w.litter_perm.domain :=
+lemma litter_map_dom_of_mem_next_image_core_domain {a : atom}
+  (h : a ∈ φ.next_image_core_domain hφ) : a.1 ∈ (φ.litter_perm hφ).domain :=
 begin
   rw next_image_core_domain at h,
   simp only [pfun.mem_dom, Union_exists, mem_Union, mem_image, mem_set_of_eq, set_coe.exists,
     subtype.coe_mk, exists_and_distrib_right, exists_eq_right, exists_prop] at h,
   obtain ⟨L, hL, ha, h⟩ := h,
-  have := (w.orbit_set_subset L ha).1,
+  have := (φ.orbit_set_subset L ha).1,
   rw mem_litter_set at this,
   rw this,
   exact hL,
 end
 
-lemma mem_orbit_set_of_mem_next_image_core_domain {a : atom} (h : a ∈ w.next_image_core_domain) :
-  a ∈ w.orbit_set a.1 :=
+lemma mem_orbit_set_of_mem_next_image_core_domain {a : atom} (h : a ∈ φ.next_image_core_domain hφ) :
+  a ∈ φ.orbit_set a.1 :=
 begin
   rw next_image_core_domain at h,
   simp only [pfun.mem_dom, Union_exists, mem_Union, mem_image, mem_set_of_eq, set_coe.exists,
     subtype.coe_mk, exists_and_distrib_right, exists_eq_right, exists_prop] at h,
   obtain ⟨L, hL, ha, h⟩ := h,
-  have := (w.orbit_set_subset L ha).1,
+  have := (φ.orbit_set_subset L ha).1,
   rw mem_litter_set at this,
   rw this,
   exact ha,
 end
 
 lemma orbit_set_equiv_elim_of_mem_next_image_core_domain {a : atom}
-  (h : a ∈ w.next_image_core_domain) :
-  (w.orbit_set_equiv a.1 ⟨a, w.mem_orbit_set_of_mem_next_image_core_domain h⟩).elim
-    (λ c, c ∈ w.next_backward_image_domain a.1) (λ c, c ∈ w.next_forward_image_domain a.1) :=
+  (h : a ∈ φ.next_image_core_domain hφ) :
+  (φ.orbit_set_equiv a.1 ⟨a, φ.mem_orbit_set_of_mem_next_image_core_domain hφ h⟩).elim
+    (λ c, c ∈ φ.next_backward_image_domain hφ a.1) (λ c, c ∈ φ.next_forward_image_domain hφ a.1) :=
 begin
   rw next_image_core_domain at h,
   simp only [pfun.mem_dom, Union_exists, mem_Union, mem_image, mem_set_of_eq, set_coe.exists,
     subtype.coe_mk, exists_and_distrib_right, exists_eq_right, exists_prop] at h,
   obtain ⟨L, hL, ha, h⟩ := h,
-  have := (w.orbit_set_subset L ha).1,
+  have := (φ.orbit_set_subset L ha).1,
   rw mem_litter_set at this,
   cases this,
   exact h,
 end
 
 lemma next_image_core_injective (a b : atom)
-  (ha : a ∈ w.next_image_core_domain) (hb : b ∈ w.next_image_core_domain)
-  (h : w.next_image_core a a.1 (w.mem_orbit_set_of_mem_next_image_core_domain ha) =
-    w.next_image_core b b.1 (w.mem_orbit_set_of_mem_next_image_core_domain hb)) : a = b :=
+  (ha : a ∈ φ.next_image_core_domain hφ) (hb : b ∈ φ.next_image_core_domain hφ)
+  (h : φ.next_image_core hφ a a.1 (φ.mem_orbit_set_of_mem_next_image_core_domain hφ ha) =
+    φ.next_image_core hφ b b.1 (φ.mem_orbit_set_of_mem_next_image_core_domain hφ hb)) : a = b :=
 begin
   rw [next_image_core, next_image_core] at h,
-  obtain ⟨a', ha'⟩ := (w.orbit_set_equiv a.fst).symm.surjective
-    ⟨a, w.mem_orbit_set_of_mem_next_image_core_domain ha⟩,
-  obtain ⟨b', hb'⟩ := (w.orbit_set_equiv b.fst).symm.surjective
-    ⟨b, w.mem_orbit_set_of_mem_next_image_core_domain hb⟩,
-  have hae := w.orbit_set_equiv_elim_of_mem_next_image_core_domain ha,
-  have hbe := w.orbit_set_equiv_elim_of_mem_next_image_core_domain hb,
+  obtain ⟨a', ha'⟩ := (φ.orbit_set_equiv a.fst).symm.surjective
+    ⟨a, φ.mem_orbit_set_of_mem_next_image_core_domain hφ ha⟩,
+  obtain ⟨b', hb'⟩ := (φ.orbit_set_equiv b.fst).symm.surjective
+    ⟨b, φ.mem_orbit_set_of_mem_next_image_core_domain hφ hb⟩,
+  have hae := φ.orbit_set_equiv_elim_of_mem_next_image_core_domain hφ ha,
+  have hbe := φ.orbit_set_equiv_elim_of_mem_next_image_core_domain hφ hb,
   simp only [← ha', ← hb', equiv.apply_symm_apply] at h hae hbe,
   obtain (⟨m, a'⟩ | ⟨m, a'⟩) := a';
   obtain (⟨n, b'⟩ | ⟨n, b'⟩) := b';
   simp only [elim_inl, elim_inr,
     mk_mem_next_backward_image_domain, mk_mem_next_forward_image_domain] at h hae hbe,
-  { cases w.next_backward_image_injective' _ _ _ _ h,
+  { cases φ.next_backward_image_injective' hφ _ _ _ _ h,
     { rw hae.2 at hbe,
       rw [subtype.ext_iff, subtype.coe_mk] at ha' hb',
       rw [← ha', ← hb', hbe.2], },
     { exact hae, },
     { exact hbe, },
-    { exact w.litter_map_dom_of_mem_next_image_core_domain ha, },
-    { exact w.litter_map_dom_of_mem_next_image_core_domain hb, }, },
-  { cases w.next_forward_image_ne_next_backward_image h.symm, },
-  { cases w.next_forward_image_ne_next_backward_image h, },
-  { cases w.next_forward_image_injective' _ _ h,
+    { exact φ.litter_map_dom_of_mem_next_image_core_domain hφ ha, },
+    { exact φ.litter_map_dom_of_mem_next_image_core_domain hφ hb, }, },
+  { cases φ.next_forward_image_ne_next_backward_image hφ h.symm, },
+  { cases φ.next_forward_image_ne_next_backward_image hφ h, },
+  { cases φ.next_forward_image_injective' hφ _ _ h,
     { rw hae.2 at hbe,
       rw [subtype.ext_iff, subtype.coe_mk] at ha' hb',
       rw [← ha', ← hb'],
-      exact w.orbit_set_equiv_symm_congr hbe.2, },
-    { exact w.litter_map_dom_of_mem_next_image_core_domain ha, },
-    { exact w.litter_map_dom_of_mem_next_image_core_domain hb, }, },
+      exact φ.orbit_set_equiv_symm_congr hbe.2, },
+    { exact φ.litter_map_dom_of_mem_next_image_core_domain hφ ha, },
+    { exact φ.litter_map_dom_of_mem_next_image_core_domain hφ hb, }, },
 end
 
 def next_image_domain : set atom :=
-(w.need_forward_images ∩ {a | a.1 ∈ w.litter_perm.domain}) ∪ w.next_image_core_domain
+(φ.need_forward_images ∩ {a | a.1 ∈ (φ.litter_perm hφ).domain}) ∪ φ.next_image_core_domain hφ
 
-noncomputable def next_image (a : atom) (ha : a ∈ w.next_image_domain) : atom :=
+noncomputable def next_image (a : atom) (ha : a ∈ φ.next_image_domain hφ) : atom :=
 ha.elim'
-  (λ ha', (w.orbit_set_equiv (w.litter_perm a.1)).symm (inr (0, ⟨a, ha'.1⟩)))
-  (w.next_image_core a a.1 ∘ w.mem_orbit_set_of_mem_next_image_core_domain)
+  (λ ha', (φ.orbit_set_equiv (φ.litter_perm hφ a.1)).symm (inr (0, ⟨a, ha'.1⟩)))
+  (φ.next_image_core hφ a a.1 ∘ φ.mem_orbit_set_of_mem_next_image_core_domain hφ)
 
-lemma next_image_domain_small : small w.next_image_domain :=
+lemma next_image_domain_small : small (φ.next_image_domain hφ) :=
 small.union
-  (small.mono (inter_subset_left _ _) w.need_forward_images_small)
-  w.next_image_core_domain_small
+  (small.mono (inter_subset_left _ _) φ.need_forward_images_small)
+  (φ.next_image_core_domain_small hφ)
 
 lemma disjoint_need_forward_images_next_image_core_domain :
-  disjoint w.need_forward_images w.next_image_core_domain :=
+  disjoint φ.need_forward_images (φ.next_image_core_domain hφ) :=
 begin
   rw set.disjoint_iff,
   rintro a ⟨ha₁, ha₂⟩,
-  exact (w.orbit_set_subset _ (w.mem_orbit_set_of_mem_next_image_core_domain ha₂)).2 (or.inr ha₁.1),
+  exact (φ.orbit_set_subset _
+    (φ.mem_orbit_set_of_mem_next_image_core_domain hφ ha₂)).2 (or.inr ha₁.1),
 end
 
 lemma next_image_eq_of_need_forward_images (a : atom)
-  (ha : a ∈ w.need_forward_images ∧ a.1 ∈ w.litter_perm.domain) :
-  w.next_image a (or.inl ha) =
-  (w.orbit_set_equiv (w.litter_perm a.1)).symm (inr (0, ⟨a, ha.1⟩)) :=
+  (ha : a ∈ φ.need_forward_images ∧ a.1 ∈ (φ.litter_perm hφ).domain) :
+  φ.next_image hφ a (or.inl ha) =
+  (φ.orbit_set_equiv (φ.litter_perm hφ a.1)).symm (inr (0, ⟨a, ha.1⟩)) :=
 or.elim'_left _ _ _ ha
 
-lemma next_image_eq_of_mem_next_image_core_domain (a : atom) (ha : a ∈ w.next_image_core_domain) :
-  w.next_image a (or.inr ha) =
-  w.next_image_core a a.1 (w.mem_orbit_set_of_mem_next_image_core_domain ha) :=
+lemma next_image_eq_of_mem_next_image_core_domain (a : atom)
+  (ha : a ∈ φ.next_image_core_domain hφ) :
+  φ.next_image hφ a (or.inr ha) =
+  φ.next_image_core hφ a a.1 (φ.mem_orbit_set_of_mem_next_image_core_domain hφ ha) :=
 begin
   refine or.elim'_right _ _ _ _,
-  exact λ h, set.disjoint_right.mp w.disjoint_need_forward_images_next_image_core_domain ha h.1,
+  exact λ h, set.disjoint_right.mp
+    (φ.disjoint_need_forward_images_next_image_core_domain hφ) ha h.1,
 end
 
 lemma orbit_set_equiv_ne_next_image_core (a b : atom)
-  (ha : a ∈ w.need_forward_images ∧ a.fst ∈ w.litter_perm.domain)
-  (hb : b ∈ w.next_image_core_domain) :
-  (((w.orbit_set_equiv (w.litter_perm a.fst)).symm) (inr (0, ⟨a, ha.1⟩)) : atom) ≠
-    w.next_image_core b b.fst (w.mem_orbit_set_of_mem_next_image_core_domain hb) :=
+  (ha : a ∈ φ.need_forward_images ∧ a.fst ∈ (φ.litter_perm hφ).domain)
+  (hb : b ∈ φ.next_image_core_domain hφ) :
+  (((φ.orbit_set_equiv (φ.litter_perm hφ a.fst)).symm) (inr (0, ⟨a, ha.1⟩)) : atom) ≠
+    φ.next_image_core hφ b b.fst (φ.mem_orbit_set_of_mem_next_image_core_domain hφ hb) :=
 begin
-  obtain ⟨b', hb'⟩ := (w.orbit_set_equiv b.fst).symm.surjective
-    ⟨b, w.mem_orbit_set_of_mem_next_image_core_domain hb⟩,
+  obtain ⟨b', hb'⟩ := (φ.orbit_set_equiv b.fst).symm.surjective
+    ⟨b, φ.mem_orbit_set_of_mem_next_image_core_domain hφ hb⟩,
   rw equiv.symm_apply_eq at hb',
   intro h,
   rw next_image_core at h,
   rw ← hb' at h,
   obtain (⟨_ | n, b'⟩ | b') := b';
   simp only [elim_inl, elim_inr, next_backward_image, next_forward_image] at h,
-  { have := w.orbit_set_subset _ ((w.orbit_set_equiv _).symm _).prop,
+  { have := φ.orbit_set_subset _ ((φ.orbit_set_equiv _).symm _).prop,
     rw h at this,
     exact this.2 (or.inl b'.prop.1), },
-  { cases (w.orbit_set_equiv_injective h).2, },
-  { cases (w.orbit_set_equiv_injective h).2, },
+  { cases (φ.orbit_set_equiv_injective h).2, },
+  { cases (φ.orbit_set_equiv_injective h).2, },
 end
 
 lemma next_image_injective (a b : atom)
-  (ha : a ∈ w.next_image_domain) (hb : b ∈ w.next_image_domain)
-  (h : w.next_image a ha = w.next_image b hb) : a = b :=
+  (ha : a ∈ φ.next_image_domain hφ) (hb : b ∈ φ.next_image_domain hφ)
+  (h : φ.next_image hφ a ha = φ.next_image hφ b hb) : a = b :=
 begin
   cases ha;
   cases hb;
   simp only [next_image_eq_of_need_forward_images,
     next_image_eq_of_mem_next_image_core_domain] at h,
-  { have := w.orbit_set_equiv_injective h,
+  { have := φ.orbit_set_equiv_injective h,
     simp only [prod.mk.inj_iff, eq_self_iff_true, subtype.mk_eq_mk, true_and] at this,
     exact this.2, },
-  { cases w.orbit_set_equiv_ne_next_image_core _ _ _ _ h, },
-  { cases w.orbit_set_equiv_ne_next_image_core _ _ _ _ h.symm, },
-  { refine w.next_image_core_injective a b ha hb h, },
+  { cases φ.orbit_set_equiv_ne_next_image_core hφ _ _ _ _ h, },
+  { cases φ.orbit_set_equiv_ne_next_image_core hφ _ _ _ _ h.symm, },
+  { refine φ.next_image_core_injective hφ a b ha hb h, },
 end
 
 noncomputable def orbit_atom_map : atom →. atom :=
 λ a, {
-  dom := (w.atom_map a).dom ∨ a ∈ w.next_image_domain,
-  get := λ h, or.elim' h (w.atom_map a).get (w.next_image a)
+  dom := (φ.atom_map a).dom ∨ a ∈ φ.next_image_domain hφ,
+  get := λ h, or.elim' h (φ.atom_map a).get (φ.next_image hφ a)
 }
 
 @[simp] lemma orbit_atom_map_dom_iff (a : atom) :
-  (w.orbit_atom_map a).dom ↔ (w.atom_map a).dom ∨ a ∈ w.next_image_domain := iff.rfl
+  (φ.orbit_atom_map hφ a).dom ↔ (φ.atom_map a).dom ∨ a ∈ φ.next_image_domain hφ := iff.rfl
 
 @[simp] lemma orbit_atom_map_dom :
-  w.orbit_atom_map.dom = w.atom_map.dom ∪ w.next_image_domain := rfl
+  (φ.orbit_atom_map hφ).dom = φ.atom_map.dom ∪ φ.next_image_domain hφ := rfl
 
-lemma disjoint_atom_map_dom_next_image_domain : disjoint w.atom_map.dom w.next_image_domain :=
+lemma disjoint_atom_map_dom_next_image_domain : disjoint φ.atom_map.dom (φ.next_image_domain hφ) :=
 begin
   rw set.disjoint_iff,
   rintros a ⟨h₁, h₂ | h₂⟩,
   { exact h₂.1.2 h₁, },
-  { exact (w.orbit_set_subset _
-      (w.mem_orbit_set_of_mem_next_image_core_domain h₂)).2 (or.inl h₁), },
+  { exact (φ.orbit_set_subset _
+      (φ.mem_orbit_set_of_mem_next_image_core_domain hφ h₂)).2 (or.inl h₁), },
 end
 
-lemma orbit_atom_map_eq_of_mem_dom (a : atom) (ha : (w.atom_map a).dom) :
-  (w.orbit_atom_map a).get (or.inl ha) = (w.atom_map a).get ha :=
+lemma orbit_atom_map_eq_of_mem_dom (a : atom) (ha : (φ.atom_map a).dom) :
+  (φ.orbit_atom_map hφ a).get (or.inl ha) = (φ.atom_map a).get ha :=
 or.elim'_left _ _ _ _
 
-lemma orbit_atom_map_eq_of_mem_next_image_domain (a : atom) (ha : a ∈ w.next_image_domain) :
-  (w.orbit_atom_map a).get (or.inr ha) = w.next_image a ha :=
-or.elim'_right _ _ _ (id set.disjoint_right.mp w.disjoint_atom_map_dom_next_image_domain ha)
+lemma orbit_atom_map_eq_of_mem_next_image_domain (a : atom) (ha : a ∈ φ.next_image_domain hφ) :
+  (φ.orbit_atom_map hφ a).get (or.inr ha) = φ.next_image hφ a ha :=
+or.elim'_right _ _ _ (id set.disjoint_right.mp (φ.disjoint_atom_map_dom_next_image_domain hφ) ha)
 
 lemma orbit_atom_map_eq_of_need_forward_images (a : atom)
-  (ha : a ∈ w.need_forward_images ∧ a.fst ∈ w.litter_perm.domain) :
-  (w.orbit_atom_map a).get (or.inr (or.inl ha)) =
-  (w.orbit_set_equiv (w.litter_perm a.1)).symm (inr (0, ⟨a, ha.1⟩)) :=
+  (ha : a ∈ φ.need_forward_images ∧ a.fst ∈ (φ.litter_perm hφ).domain) :
+  (φ.orbit_atom_map hφ a).get (or.inr (or.inl ha)) =
+  (φ.orbit_set_equiv (φ.litter_perm hφ a.1)).symm (inr (0, ⟨a, ha.1⟩)) :=
 begin
   unfold orbit_atom_map,
   simp only,
   rw or.elim'_right,
-  exact w.next_image_eq_of_need_forward_images a ha,
-  exact id set.disjoint_right.mp w.disjoint_atom_map_dom_next_image_domain (or.inl ha),
+  exact φ.next_image_eq_of_need_forward_images hφ a ha,
+  exact id set.disjoint_right.mp (φ.disjoint_atom_map_dom_next_image_domain hφ) (or.inl ha),
 end
 
 lemma orbit_atom_map_eq_of_mem_next_image_core_domain (a : atom)
-  (ha : a ∈ w.next_image_core_domain) :
-  (w.orbit_atom_map a).get (or.inr (or.inr ha)) =
-    w.next_image_core a a.1 (w.mem_orbit_set_of_mem_next_image_core_domain ha) :=
+  (ha : a ∈ φ.next_image_core_domain hφ) :
+  (φ.orbit_atom_map hφ a).get (or.inr (or.inr ha)) =
+    φ.next_image_core hφ a a.1 (φ.mem_orbit_set_of_mem_next_image_core_domain hφ ha) :=
 begin
   unfold orbit_atom_map,
   simp only,
   rw or.elim'_right,
-  exact w.next_image_eq_of_mem_next_image_core_domain a ha,
-  exact id set.disjoint_right.mp w.disjoint_atom_map_dom_next_image_domain (or.inr ha),
+  exact φ.next_image_eq_of_mem_next_image_core_domain hφ a ha,
+  exact id set.disjoint_right.mp (φ.disjoint_atom_map_dom_next_image_domain hφ) (or.inr ha),
 end
 
-lemma orbit_atom_map_dom_small : small w.orbit_atom_map.dom :=
-small.union w.atom_map_dom_small w.next_image_domain_small
+lemma orbit_atom_map_dom_small : small (φ.orbit_atom_map hφ).dom :=
+small.union φ.atom_map_dom_small (φ.next_image_domain_small hφ)
 
 lemma orbit_atom_map_apply_ne_of_need_forward_images ⦃a b : atom⦄
-  (ha : (w.atom_map a).dom) (hb : b ∈ w.need_forward_images ∧ b.fst ∈ w.litter_perm.domain) :
-  (w.orbit_atom_map a).get (or.inl ha) ≠ (w.orbit_atom_map b).get (or.inr (or.inl hb)) :=
+  (ha : (φ.atom_map a).dom) (hb : b ∈ φ.need_forward_images ∧ b.fst ∈ (φ.litter_perm hφ).domain) :
+  (φ.orbit_atom_map hφ a).get (or.inl ha) ≠ (φ.orbit_atom_map hφ b).get (or.inr (or.inl hb)) :=
 begin
   rw [orbit_atom_map_eq_of_mem_dom, orbit_atom_map_eq_of_need_forward_images],
   intro h,
-  have := w.orbit_set_subset _ ((w.orbit_set_equiv _).symm _).prop,
+  have := φ.orbit_set_subset _ ((φ.orbit_set_equiv _).symm _).prop,
   rw ← h at this,
   exact this.2 (or.inr ⟨a, ha, rfl⟩),
 end
 
 lemma orbit_atom_map_apply_ne_of_mem_next_image_core_domain ⦃a b : atom⦄
-  (ha : (w.atom_map a).dom) (hb : b ∈ w.next_image_core_domain) :
-  (w.orbit_atom_map a).get (or.inl ha) ≠ (w.orbit_atom_map b).get (or.inr (or.inr hb)) :=
+  (ha : (φ.atom_map a).dom) (hb : b ∈ φ.next_image_core_domain hφ) :
+  (φ.orbit_atom_map hφ a).get (or.inl ha) ≠ (φ.orbit_atom_map hφ b).get (or.inr (or.inr hb)) :=
 begin
-  obtain ⟨b', hb'⟩ := (w.orbit_set_equiv b.fst).symm.surjective
-    ⟨b, w.mem_orbit_set_of_mem_next_image_core_domain hb⟩,
+  obtain ⟨b', hb'⟩ := (φ.orbit_set_equiv b.fst).symm.surjective
+    ⟨b, φ.mem_orbit_set_of_mem_next_image_core_domain hφ hb⟩,
   rw [orbit_atom_map_eq_of_mem_dom, orbit_atom_map_eq_of_mem_next_image_core_domain,
     next_image_core, ← hb', equiv.apply_symm_apply],
   obtain (⟨_ | n, b'⟩ | ⟨n, b'⟩) := b';
@@ -489,49 +492,50 @@ begin
     rw ← h at this,
     exact this ⟨a, ha, rfl⟩, },
   { intro h,
-    have := (w.orbit_set_subset _ ((w.orbit_set_equiv _).symm _).prop).2,
+    have := (φ.orbit_set_subset _ ((φ.orbit_set_equiv _).symm _).prop).2,
     rw ← h at this,
     exact this (or.inr ⟨a, ha, rfl⟩), },
   { intro h,
-    have := (w.orbit_set_subset _ ((w.orbit_set_equiv _).symm _).prop).2,
+    have := (φ.orbit_set_subset _ ((φ.orbit_set_equiv _).symm _).prop).2,
     rw ← h at this,
     exact this (or.inr ⟨a, ha, rfl⟩), },
 end
 
 lemma orbit_atom_map_apply_ne ⦃a b : atom⦄
-  (ha : (w.atom_map a).dom) (hb : b ∈ w.next_image_domain) :
-  (w.orbit_atom_map a).get (or.inl ha) ≠ (w.orbit_atom_map b).get (or.inr hb) :=
+  (ha : (φ.atom_map a).dom) (hb : b ∈ φ.next_image_domain hφ) :
+  (φ.orbit_atom_map hφ a).get (or.inl ha) ≠ (φ.orbit_atom_map hφ b).get (or.inr hb) :=
 begin
   cases hb,
-  exact w.orbit_atom_map_apply_ne_of_need_forward_images ha hb,
-  exact w.orbit_atom_map_apply_ne_of_mem_next_image_core_domain ha hb,
+  exact φ.orbit_atom_map_apply_ne_of_need_forward_images hφ ha hb,
+  exact φ.orbit_atom_map_apply_ne_of_mem_next_image_core_domain hφ ha hb,
 end
 
 lemma orbit_atom_map_injective ⦃a b : atom⦄
-  (ha : (w.orbit_atom_map a).dom) (hb : (w.orbit_atom_map b).dom)
-  (h : (w.orbit_atom_map a).get ha = (w.orbit_atom_map b).get hb) : a = b :=
+  (ha : (φ.orbit_atom_map hφ a).dom) (hb : (φ.orbit_atom_map hφ b).dom)
+  (h : (φ.orbit_atom_map hφ a).get ha = (φ.orbit_atom_map hφ b).get hb) :
+  a = b :=
 begin
   cases ha;
   cases hb,
   { rw [orbit_atom_map_eq_of_mem_dom, orbit_atom_map_eq_of_mem_dom] at h,
-    exact w.atom_map_injective ha hb h, },
-  { cases w.orbit_atom_map_apply_ne ha hb h, },
-  { cases w.orbit_atom_map_apply_ne hb ha h.symm, },
+    exact hφ.atom_map_injective ha hb h, },
+  { cases φ.orbit_atom_map_apply_ne hφ ha hb h, },
+  { cases φ.orbit_atom_map_apply_ne hφ hb ha h.symm, },
   { rw [orbit_atom_map_eq_of_mem_next_image_domain,
       orbit_atom_map_eq_of_mem_next_image_domain] at h,
-    exact w.next_image_injective a b ha hb h, },
+    exact φ.next_image_injective hφ a b ha hb h, },
 end
 
 lemma next_image_core_atom_mem_litter_map
-  (a : atom) (ha : a ∈ w.next_image_core_domain) :
-  w.next_image_core a a.fst (w.mem_orbit_set_of_mem_next_image_core_domain ha) ∈
-    litter_set (w.litter_perm a.fst) :=
+  (a : atom) (ha : a ∈ φ.next_image_core_domain hφ) :
+  φ.next_image_core hφ a a.fst (φ.mem_orbit_set_of_mem_next_image_core_domain hφ ha) ∈
+    litter_set (φ.litter_perm hφ a.fst) :=
 begin
-  have hL := w.litter_map_dom_of_mem_next_image_core_domain ha,
-  have := w.mem_orbit_set_of_mem_next_image_core_domain ha,
-  obtain ⟨a', ha'⟩ := (w.orbit_set_equiv a.fst).symm.surjective
-    ⟨a, w.mem_orbit_set_of_mem_next_image_core_domain ha⟩,
-  have := w.orbit_set_equiv_elim_of_mem_next_image_core_domain ha,
+  have hL := φ.litter_map_dom_of_mem_next_image_core_domain hφ ha,
+  have := φ.mem_orbit_set_of_mem_next_image_core_domain hφ ha,
+  obtain ⟨a', ha'⟩ := (φ.orbit_set_equiv a.fst).symm.surjective
+    ⟨a, φ.mem_orbit_set_of_mem_next_image_core_domain hφ ha⟩,
+  have := φ.orbit_set_equiv_elim_of_mem_next_image_core_domain hφ ha,
   rw [next_image_core],
   rw [← ha', equiv.apply_symm_apply] at this ⊢,
   obtain (⟨_ | n, a'⟩ | ⟨n, a'⟩) := a';
@@ -543,73 +547,74 @@ begin
     { exact ha''.symm, },
     { exact hL, },
     { exact this.1, }, },
-  exact (w.orbit_set_subset _ ((w.orbit_set_equiv _).symm _).prop).1,
-  exact (w.orbit_set_subset _ ((w.orbit_set_equiv _).symm _).prop).1,
+  exact (φ.orbit_set_subset _ ((φ.orbit_set_equiv _).symm _).prop).1,
+  exact (φ.orbit_set_subset _ ((φ.orbit_set_equiv _).symm _).prop).1,
 end
 
 lemma next_image_core_not_mem_ran
-  (a : atom) (ha : a ∈ w.next_image_core_domain) :
-  w.next_image_core a a.fst (w.mem_orbit_set_of_mem_next_image_core_domain ha) ∉ w.atom_map.ran :=
+  (a : atom) (ha : a ∈ φ.next_image_core_domain hφ) :
+  φ.next_image_core hφ a a.fst (φ.mem_orbit_set_of_mem_next_image_core_domain hφ ha) ∉
+    φ.atom_map.ran :=
 begin
   rintro ⟨b, hb₁, hb₂⟩,
   rw next_image_core at hb₂,
-  obtain ⟨a', ha'⟩ := (w.orbit_set_equiv a.fst).symm.surjective
-    ⟨a, w.mem_orbit_set_of_mem_next_image_core_domain ha⟩,
+  obtain ⟨a', ha'⟩ := (φ.orbit_set_equiv a.fst).symm.surjective
+    ⟨a, φ.mem_orbit_set_of_mem_next_image_core_domain hφ ha⟩,
   rw [← ha', equiv.apply_symm_apply] at hb₂,
   obtain (⟨_ | n, a'⟩ | ⟨n, a'⟩) := a';
   simp only [elim_inr, elim_inl, nat.nat_zero_eq_zero, next_backward_image, next_forward_image,
     mk_mem_next_backward_image_domain, mk_mem_next_forward_image_domain,
     function.iterate_one] at hb₂,
   { exact a'.prop.2 ⟨b, hb₁, hb₂⟩, },
-  all_goals { have := w.orbit_set_subset _ ((w.orbit_set_equiv _).symm _).prop,
+  all_goals { have := φ.orbit_set_subset _ ((φ.orbit_set_equiv _).symm _).prop,
     rw ← hb₂ at this,
     exact this.2 (or.inr ⟨b, hb₁, rfl⟩), },
 end
 
 lemma next_image_core_atom_mem
-  (hdiff : ∀ L hL, ((w.litter_map L).get hL : set atom) ∆ litter_set ((w.litter_map L).get hL).1 ⊆
-    w.atom_map.ran)
-  (a : atom) (ha : a ∈ w.next_image_core_domain)
-  (L : litter) (hL : (w.litter_map L).dom) :
+  (hdiff : ∀ L hL, ((φ.litter_map L).get hL : set atom) ∆ litter_set ((φ.litter_map L).get hL).1 ⊆
+    φ.atom_map.ran)
+  (a : atom) (ha : a ∈ φ.next_image_core_domain hφ)
+  (L : litter) (hL : (φ.litter_map L).dom) :
   a.fst = L ↔
-    w.next_image_core a a.fst (w.mem_orbit_set_of_mem_next_image_core_domain ha) ∈
-      (w.litter_map L).get hL :=
+    φ.next_image_core hφ a a.fst (φ.mem_orbit_set_of_mem_next_image_core_domain hφ ha) ∈
+      (φ.litter_map L).get hL :=
 begin
-  have hamem := w.mem_orbit_set_of_mem_next_image_core_domain ha,
-  have ha' := w.next_image_core_atom_mem_litter_map a ha,
+  have hamem := φ.mem_orbit_set_of_mem_next_image_core_domain hφ ha,
+  have ha' := φ.next_image_core_atom_mem_litter_map hφ a ha,
   rw mem_litter_set at ha',
   split,
   { rintro rfl,
-    have := not_mem_subset (hdiff _ hL) (w.next_image_core_not_mem_ran a ha),
+    have := not_mem_subset (hdiff _ hL) (φ.next_image_core_not_mem_ran hφ a ha),
     simp only [mem_symm_diff, set_like.mem_coe, mem_litter_set,
       not_or_distrib, not_and_distrib, not_not] at this,
     refine this.2.resolve_left (not_not.mpr _),
     rw ha',
-    rw w.litter_perm_apply_eq _ hL,
-    rw w.rough_litter_map_or_else_of_dom,  },
+    rw litter_perm_apply_eq _ hL,
+    rw φ.rough_litter_map_or_else_of_dom,  },
   { intro h,
-    have hL' := w.litter_perm_apply_eq L hL,
-    rw w.rough_litter_map_or_else_of_dom hL at hL',
-    have := not_mem_subset (hdiff _ hL) (w.next_image_core_not_mem_ran a ha),
+    have hL' := litter_perm_apply_eq L hL,
+    rw φ.rough_litter_map_or_else_of_dom hL at hL',
+    have := not_mem_subset (hdiff _ hL) (φ.next_image_core_not_mem_ran hφ a ha),
     simp only [mem_symm_diff, set_like.mem_coe, mem_litter_set, not_not, h, true_and,
       not_true, and_false, or_false] at this,
     rw [ha', ← hL', ← local_perm.eq_symm_apply, local_perm.left_inv] at this,
     exact this,
     exact or.inl (or.inl (or.inl hL)),
-    exact w.litter_map_dom_of_mem_next_image_core_domain ha,
+    exact φ.litter_map_dom_of_mem_next_image_core_domain hφ ha,
     exact local_perm.map_domain _ (or.inl (or.inl (or.inl hL))), },
 end
 
 lemma orbit_set_equiv_atom_mem
-  (hdiff : ∀ L hL, ((w.litter_map L).get hL : set atom) ∆ litter_set ((w.litter_map L).get hL).1 ⊆
-    w.atom_map.ran)
-  (a : atom) (ha : a ∈ w.need_forward_images ∧ a.fst ∈ w.litter_perm.domain)
-  (L : litter) (hL : (w.litter_map L).dom) :
-  a.fst = L ↔ ((w.orbit_set_equiv (w.litter_perm a.fst)).symm (inr (0, ⟨a, ha.1⟩)) : atom) ∈
-    (w.litter_map L).get hL :=
+  (hdiff : ∀ L hL, ((φ.litter_map L).get hL : set atom) ∆ litter_set ((φ.litter_map L).get hL).1 ⊆
+    φ.atom_map.ran)
+  (a : atom) (ha : a ∈ φ.need_forward_images ∧ a.fst ∈ (φ.litter_perm hφ).domain)
+  (L : litter) (hL : (φ.litter_map L).dom) :
+  a.fst = L ↔ ((φ.orbit_set_equiv (φ.litter_perm hφ a.fst)).symm (inr (0, ⟨a, ha.1⟩)) : atom) ∈
+    (φ.litter_map L).get hL :=
 begin
-  have ha' : _ ∧ _ := w.orbit_set_subset _
-    ((w.orbit_set_equiv (w.litter_perm a.fst)).symm (inr (0, ⟨a, ha.1⟩))).prop,
+  have ha' : _ ∧ _ := φ.orbit_set_subset _
+    ((φ.orbit_set_equiv (φ.litter_perm hφ a.fst)).symm (inr (0, ⟨a, ha.1⟩))).prop,
   rw mem_litter_set at ha',
   split,
   { rintro rfl,
@@ -618,152 +623,155 @@ begin
       not_or_distrib, not_and_distrib, not_not] at this,
     refine this.2.resolve_left (not_not.mpr _),
     { rw ha'.1,
-      rw w.litter_perm_apply_eq _ hL,
-      rw w.rough_litter_map_or_else_of_dom, },
+      rw litter_perm_apply_eq _ hL,
+      rw φ.rough_litter_map_or_else_of_dom, },
     { exact ha'.2 ∘ or.inr, }, },
   { intro h,
     have := @not_mem_subset _
-      ((w.orbit_set_equiv (w.litter_perm a.fst)).symm (inr (0, ⟨a, ha.1⟩)) : atom) _ _
+      ((φ.orbit_set_equiv (φ.litter_perm hφ a.fst)).symm (inr (0, ⟨a, ha.1⟩)) : atom) _ _
       (hdiff L hL) (ha'.2 ∘ or.inr),
     simp only [mem_symm_diff, h, set_like.mem_coe, mem_litter_set, true_and, not_true, and_false,
       or_false, not_not] at this,
-    rw [ha'.1, ← rough_litter_map_or_else_of_dom, ← litter_perm_apply_eq,
+    rw [ha'.1, ← rough_litter_map_or_else_of_dom, ← @litter_perm_apply_eq _ _ hφ,
       ← local_perm.eq_symm_apply, local_perm.left_inv] at this,
     exact this,
     { exact or.inl (or.inl (or.inl hL)), },
     { exact ha.2, },
-    { exact w.litter_perm.map_domain (or.inl (or.inl (or.inl hL))), },
+    { exact (φ.litter_perm hφ).map_domain (or.inl (or.inl (or.inl hL))), },
     { exact hL, }, },
 end
 
 lemma orbit_atom_mem
-  (hdiff : ∀ L hL, ((w.litter_map L).get hL : set atom) ∆ litter_set ((w.litter_map L).get hL).1 ⊆
-    w.atom_map.ran)
-  (a : atom) (ha : (w.orbit_atom_map a).dom)
-  (L : litter) (hL : (w.litter_map L).dom) :
-  a.fst = L ↔ (w.orbit_atom_map a).get ha ∈ (w.litter_map L).get hL :=
+  (hdiff : ∀ L hL, ((φ.litter_map L).get hL : set atom) ∆ litter_set ((φ.litter_map L).get hL).1 ⊆
+    φ.atom_map.ran)
+  (a : atom) (ha : (φ.orbit_atom_map hφ a).dom)
+  (L : litter) (hL : (φ.litter_map L).dom) :
+  a.fst = L ↔ (φ.orbit_atom_map hφ a).get ha ∈ (φ.litter_map L).get hL :=
 begin
   obtain ha | ha | ha := ha,
   { rw orbit_atom_map_eq_of_mem_dom,
-    exact w.atom_mem a ha L hL, },
+    exact hφ.atom_mem a ha L hL, },
   { rw orbit_atom_map_eq_of_need_forward_images,
-    exact w.orbit_set_equiv_atom_mem hdiff a ha L hL, },
+    exact φ.orbit_set_equiv_atom_mem hφ hdiff a ha L hL, },
   { rw orbit_atom_map_eq_of_mem_next_image_core_domain,
-    rw w.next_image_core_atom_mem hdiff a ha L hL, },
+    rw φ.next_image_core_atom_mem hφ hdiff a ha L hL, },
 end
 
-noncomputable def fill_atom_orbits
-  (hdiff : ∀ L hL, ((w.litter_map L).get hL : set atom) ∆ litter_set ((w.litter_map L).get hL).1 ⊆
-    w.atom_map.ran) : weak_near_litter_approx := {
-  atom_map := w.orbit_atom_map,
-  litter_map := w.litter_map,
-  atom_map_dom_small := w.orbit_atom_map_dom_small,
-  litter_map_dom_small := w.litter_map_dom_small,
-  atom_map_injective := w.orbit_atom_map_injective,
-  litter_map_injective := w.litter_map_injective,
-  atom_mem := w.orbit_atom_mem hdiff,
+noncomputable def fill_atom_orbits : near_litter_action := {
+  atom_map := φ.orbit_atom_map hφ,
+  litter_map := φ.litter_map,
+  atom_map_dom_small := φ.orbit_atom_map_dom_small hφ,
+  litter_map_dom_small := φ.litter_map_dom_small,
 }
 
-variables {w} {hdiff : ∀ L hL,
-  ((w.litter_map L).get hL : set atom) ∆ litter_set ((w.litter_map L).get hL).1 ⊆ w.atom_map.ran}
+lemma fill_atom_orbits_lawful
+  (hdiff : ∀ L hL, ((φ.litter_map L).get hL : set atom) ∆ litter_set ((φ.litter_map L).get hL).1 ⊆
+    φ.atom_map.ran) : (φ.fill_atom_orbits hφ).lawful := {
+  atom_map_injective := φ.orbit_atom_map_injective hφ,
+  litter_map_injective := hφ.litter_map_injective,
+  atom_mem := φ.orbit_atom_mem hφ hdiff,
+}
+
+variables {φ} {hdiff : ∀ L hL,
+  ((φ.litter_map L).get hL : set atom) ∆ litter_set ((φ.litter_map L).get hL).1 ⊆ φ.atom_map.ran}
 
 @[simp] lemma fill_atom_orbits_atom_map :
-  (w.fill_atom_orbits hdiff).atom_map = w.orbit_atom_map := rfl
+  (φ.fill_atom_orbits hφ).atom_map = φ.orbit_atom_map hφ := rfl
 
 @[simp] lemma fill_atom_orbits_litter_map :
-  (w.fill_atom_orbits hdiff).litter_map = w.litter_map := rfl
+  (φ.fill_atom_orbits hφ).litter_map = φ.litter_map := rfl
 
-lemma subset_orbit_atom_map_dom : w.atom_map.dom ⊆ w.orbit_atom_map.dom :=
+lemma subset_orbit_atom_map_dom : φ.atom_map.dom ⊆ (φ.orbit_atom_map hφ).dom :=
 subset_union_left _ _
 
-lemma subset_orbit_atom_map_ran : w.atom_map.ran ⊆ w.orbit_atom_map.ran :=
+lemma subset_orbit_atom_map_ran : φ.atom_map.ran ⊆ (φ.orbit_atom_map hφ).ran :=
 begin
   rintro _ ⟨a, ha, rfl⟩,
-  exact ⟨a, subset_orbit_atom_map_dom ha, w.orbit_atom_map_eq_of_mem_dom _ _⟩,
+  exact ⟨a, subset_orbit_atom_map_dom hφ ha, φ.orbit_atom_map_eq_of_mem_dom hφ _ _⟩,
 end
 
-lemma fst_mem_litter_perm_domain_of_mem_map ⦃L : litter⦄ (hL : (w.litter_map L).dom)
-  ⦃a : atom⦄ (ha : a ∈ (w.litter_map L).get hL) :
-  a.1 ∈ w.litter_perm.domain :=
+lemma fst_mem_litter_perm_domain_of_mem_map ⦃L : litter⦄ (hL : (φ.litter_map L).dom)
+  ⦃a : atom⦄ (ha : a ∈ (φ.litter_map L).get hL) :
+  a.1 ∈ (φ.litter_perm hφ).domain :=
 begin
-  by_cases a.1 = ((w.litter_map L).get hL).1,
+  by_cases a.1 = ((φ.litter_map L).get hL).1,
   { rw h,
     refine or.inl (or.inl (or.inr ⟨L, hL, _⟩)),
     rw rough_litter_map_or_else_of_dom, },
-  { by_cases h' : a.fst ∈ w.litter_perm'.domain,
+  { by_cases h' : a.fst ∈ (φ.litter_perm' hφ).domain,
     exact or.inl h',
     exact or.inr ⟨banned_litter.diff L hL a ⟨ha, h⟩, h'⟩, },
 end
 
-lemma fst_mem_litter_perm_domain_of_dom ⦃a : atom⦄ (ha : a ∈ w.atom_map.dom) :
-  a.fst ∈ w.litter_perm.domain :=
+lemma fst_mem_litter_perm_domain_of_dom ⦃a : atom⦄ (ha : a ∈ φ.atom_map.dom) :
+  a.fst ∈ (φ.litter_perm hφ).domain :=
 begin
-  by_cases h' : a.fst ∈ w.litter_perm'.domain,
+  by_cases h' : a.fst ∈ (φ.litter_perm' hφ).domain,
   exact or.inl h',
   exact or.inr ⟨banned_litter.atom_dom a ha, h'⟩,
 end
 
-lemma fst_mem_litter_perm_domain_of_ran ⦃a : atom⦄ (ha : a ∈ w.atom_map.ran) :
-  a.fst ∈ w.litter_perm.domain :=
+lemma fst_mem_litter_perm_domain_of_ran ⦃a : atom⦄ (ha : a ∈ φ.atom_map.ran) :
+  a.fst ∈ (φ.litter_perm hφ).domain :=
 begin
-  by_cases h' : a.fst ∈ w.litter_perm'.domain,
+  by_cases h' : a.fst ∈ (φ.litter_perm' hφ).domain,
   exact or.inl h',
   obtain ⟨b, hb, rfl⟩ := ha,
   exact or.inr ⟨banned_litter.atom_map b hb, h'⟩,
 end
 
 lemma fill_atom_orbits_precise
-  (hdiff : ∀ L hL, ((w.litter_map L).get hL : set atom) ∆ litter_set ((w.litter_map L).get hL).1 ⊆
-    w.atom_map.ran) : precise (w.fill_atom_orbits hdiff) :=
+  (hdiff : ∀ L hL, ((φ.litter_map L).get hL : set atom) ∆ litter_set ((φ.litter_map L).get hL).1 ⊆
+    φ.atom_map.ran) : precise (φ.fill_atom_orbits hφ) :=
 begin
   intros L hL,
   constructor,
-  { exact subset_trans (hdiff L hL) subset_orbit_atom_map_ran, },
+  { exact subset_trans (hdiff L hL) (subset_orbit_atom_map_ran hφ), },
   { intros a ha ha',
     simp only [fill_atom_orbits_atom_map, fill_atom_orbits_litter_map, mem_litter_set,
       orbit_atom_map_dom_iff] at *,
     obtain ha | ha | ha := ha,
-    { have := w.orbit_atom_map_eq_of_mem_dom a ha,
+    { have := φ.orbit_atom_map_eq_of_mem_dom hφ a ha,
       generalize_proofs at this ha' ⊢,
       rw [this, or_iff_not_imp_left],
       intro hmap,
-      have hfwd : (w.atom_map a).get ha ∈ w.need_forward_images := ⟨⟨a, _, rfl⟩, hmap⟩,
+      have hfwd : (φ.atom_map a).get ha ∈ φ.need_forward_images := ⟨⟨a, _, rfl⟩, hmap⟩,
       refine or.inl ⟨hfwd, or.inl (or.inl _)⟩,
       refine mem_of_eq_of_mem _ (or.inl hL),
       rw [← ha', this], },
     { refine or.inr (or.inr ⟨_, ⟨L, rfl⟩, _⟩),
       simp only [pfun.mem_dom, Union_exists, mem_Union, mem_image, mem_set_of_eq, set_coe.exists,
         subtype.coe_mk, exists_and_distrib_right, exists_eq_right, exists_prop],
-      have haL : L = w.litter_perm a.fst,
+      have haL : L = φ.litter_perm hφ a.fst,
       { have := (congr_arg prod.fst
-          (w.orbit_atom_map_eq_of_need_forward_images a ha)).symm.trans ha',
+          (φ.orbit_atom_map_eq_of_need_forward_images hφ a ha)).symm.trans ha',
         rw ← this,
-        exact (w.orbit_set_subset _ ((w.orbit_set_equiv _).symm _).prop).1, },
+        exact (φ.orbit_set_subset _ ((φ.orbit_set_equiv _).symm _).prop).1, },
       refine ⟨or.inl (or.inl (or.inl hL)), _, _⟩,
-      { refine mem_of_eq_of_mem (w.orbit_atom_map_eq_of_need_forward_images a ha) _,
+      { refine mem_of_eq_of_mem (φ.orbit_atom_map_eq_of_need_forward_images hφ a ha) _,
         rw haL,
-        exact ((w.orbit_set_equiv _).symm _).prop, },
-      { have := w.orbit_atom_map_eq_of_need_forward_images a ha,
+        exact ((φ.orbit_set_equiv _).symm _).prop, },
+      { have := φ.orbit_atom_map_eq_of_need_forward_images hφ a ha,
         obtain ⟨hm₁, hm₂⟩ := subtype.coe_eq_iff.mp this.symm,
-        rw [equiv.symm_apply_eq, w.orbit_set_equiv_congr hm₁ haL.symm] at hm₂,
+        rw [equiv.symm_apply_eq, φ.orbit_set_equiv_congr hm₁ haL.symm] at hm₂,
         refine mem_of_eq_of_mem hm₂.symm _,
-        change sum.elim (λ b, b ∈ w.next_backward_image_domain L)
-          (λ b, b ∈ w.next_forward_image_domain L) (inr (0, ⟨a, ha.1⟩)),
+        change sum.elim (λ b, b ∈ φ.next_backward_image_domain hφ L)
+          (λ b, b ∈ φ.next_forward_image_domain hφ L) (inr (0, ⟨a, ha.1⟩)),
         refine ⟨ha.2, _⟩,
         simp only [subtype.coe_mk, function.iterate_one],
         exact haL.symm, }, },
-    { have := w.orbit_atom_map_eq_of_mem_next_image_core_domain a ha,
+    { have := φ.orbit_atom_map_eq_of_mem_next_image_core_domain hφ a ha,
       generalize_proofs at this ha' ⊢,
       rw [this, next_image_core],
       obtain ⟨_, ⟨L', rfl⟩, _, ⟨hL', rfl⟩, a, hbL, rfl⟩ := ha,
-      set b := w.orbit_set_equiv L' a with hb,
+      set b := φ.orbit_set_equiv L' a with hb,
       clear_value b,
       simp only [mem_set_of_eq] at hbL,
       rw ← hb at hbL,
-      have haL' := (w.orbit_set_subset _ a.prop).1,
+      have haL' := (φ.orbit_set_subset _ a.prop).1,
       rw mem_litter_set at haL',
-      have := w.orbit_set_equiv_congr (w.mem_orbit_set_of_mem_next_image_core_domain _)
-        (w.orbit_set_subset _ a.prop).1,
+      have := φ.orbit_set_equiv_congr (φ.mem_orbit_set_of_mem_next_image_core_domain hφ _)
+        (φ.orbit_set_subset _ a.prop).1,
       rw subtype.coe_eta at this,
       rw [this, ← hb],
       obtain (⟨_ | n, b⟩ | ⟨n, b⟩) := b;
@@ -774,32 +782,32 @@ begin
         have hbL' := hbL.2,
         symmetry' at hbL',
         rw [function.iterate_succ_apply',
-          local_perm.eq_symm_apply _ hL' (w.litter_perm.symm.iterate_domain hbL.1)] at hbL',
-        refine ⟨_, ⟨w.litter_perm.symm^[n + 1] (b : atom).1, rfl⟩, _, ⟨_, rfl⟩,
-          ⟨(w.orbit_set_equiv (w.litter_perm (a : atom).1)).symm (inl (n, b)), _⟩, _⟩,
-        { exact w.litter_perm.symm.iterate_domain hbL.1, },
+          local_perm.eq_symm_apply _ hL' ((φ.litter_perm hφ).symm.iterate_domain hbL.1)] at hbL',
+        refine ⟨_, ⟨(φ.litter_perm hφ).symm^[n + 1] (b : atom).1, rfl⟩, _, ⟨_, rfl⟩,
+          ⟨(φ.orbit_set_equiv (φ.litter_perm hφ (a : atom).1)).symm (inl (n, b)), _⟩, _⟩,
+        { exact (φ.litter_perm hφ).symm.iterate_domain hbL.1, },
         { rw ← hbL',
-          have := (((w.orbit_set_equiv (w.litter_perm (a : atom).1)).symm (inl (n, b)))).prop,
+          have := (((φ.orbit_set_equiv (φ.litter_perm hφ (a : atom).1)).symm (inl (n, b)))).prop,
           rw haL' at this ⊢,
           exact this, },
         { simp only [function.comp_app, mem_set_of_eq, subtype.coe_mk,
             eq_self_iff_true, and_true],
-          rw [w.orbit_set_equiv_congr _ hbL'.symm,
-            w.orbit_set_equiv_congr _ (congr_arg w.litter_perm haL'.symm)],
+          rw [φ.orbit_set_equiv_congr _ hbL'.symm,
+            φ.orbit_set_equiv_congr _ (congr_arg (φ.litter_perm hφ) haL'.symm)],
           simp only [subtype.coe_eta, equiv.apply_symm_apply, elim_inl],
           exact ⟨hbL.1, rfl⟩, }, },
       { refine or.inr (or.inr _),
-        refine ⟨_, ⟨w.litter_perm^[n + 2] (b : atom).1, rfl⟩, _, ⟨_, rfl⟩,
-          ⟨(w.orbit_set_equiv (w.litter_perm (a : atom).1)).symm (inr (n + 1, b)), _⟩, _⟩,
-        { exact w.litter_perm.iterate_domain hbL.1, },
+        refine ⟨_, ⟨(φ.litter_perm hφ)^[n + 2] (b : atom).1, rfl⟩, _, ⟨_, rfl⟩,
+          ⟨(φ.orbit_set_equiv (φ.litter_perm hφ (a : atom).1)).symm (inr (n + 1, b)), _⟩, _⟩,
+        { exact (φ.litter_perm hφ).iterate_domain hbL.1, },
         { rw [function.iterate_succ_apply', hbL.2, haL'],
-          exact ((w.orbit_set_equiv _).symm _).prop, },
+          exact ((φ.orbit_set_equiv _).symm _).prop, },
         { simp only [function.comp_app, mem_set_of_eq,
             subtype.coe_mk, eq_self_iff_true, and_true],
-          have := congr_arg w.litter_perm hbL.2,
-          rw ← function.iterate_succ_apply' w.litter_perm (n + 1) at this,
-          rw [w.orbit_set_equiv_congr _ this,
-            w.orbit_set_equiv_congr _ (congr_arg w.litter_perm haL'.symm)],
+          have := congr_arg (φ.litter_perm hφ) hbL.2,
+          rw ← function.iterate_succ_apply' (φ.litter_perm hφ) (n + 1) at this,
+          rw [φ.orbit_set_equiv_congr _ this,
+            φ.orbit_set_equiv_congr _ (congr_arg (φ.litter_perm hφ) haL'.symm)],
           simp only [function.iterate_succ, function.comp_app, subtype.coe_eta,
             equiv.apply_symm_apply, elim_inr],
           exact ⟨hbL.1, rfl⟩, }, },
@@ -810,91 +818,94 @@ begin
     rintros a ⟨ha₁ | ⟨ha₁, ha₁'⟩ | ha₁, ha₂⟩;
     simp only [fill_atom_orbits_atom_map, fill_atom_orbits_litter_map, orbit_atom_map_dom,
       mem_inter_iff, mem_union, set_like.mem_coe] at *,
-    { by_cases ha₃ : a ∈ w.atom_map.ran,
+    { by_cases ha₃ : a ∈ φ.atom_map.ran,
       { obtain ⟨b, hb₁, hb₂⟩ := ha₃,
         refine ⟨b, or.inl hb₁, _⟩,
         rw orbit_atom_map_eq_of_mem_dom,
         exact hb₂, },
-      { refine ⟨(w.orbit_set_equiv (w.litter_perm.symm a.1)).symm (inl (0, ⟨a, ha₁, ha₃⟩)), _, _⟩,
-        { refine or.inr (or.inr ⟨_, ⟨w.litter_perm.symm a.1, rfl⟩, _, ⟨_, rfl⟩, _⟩),
-          { exact w.litter_perm.symm.map_domain (fst_mem_litter_perm_domain_of_mem_map hL ha₂), },
+      { refine ⟨(φ.orbit_set_equiv ((φ.litter_perm hφ).symm a.1)).symm
+          (inl (0, ⟨a, ha₁, ha₃⟩)), _, _⟩,
+        { refine or.inr (or.inr ⟨_, ⟨(φ.litter_perm hφ).symm a.1, rfl⟩, _, ⟨_, rfl⟩, _⟩),
+          { exact (φ.litter_perm hφ).symm.map_domain
+              (fst_mem_litter_perm_domain_of_mem_map hφ hL ha₂), },
           refine ⟨_, _, rfl⟩,
           simp only [mem_set_of_eq, equiv.apply_symm_apply, elim_inl],
-          exact ⟨fst_mem_litter_perm_domain_of_mem_map hL ha₂, rfl⟩, },
+          exact ⟨fst_mem_litter_perm_domain_of_mem_map hφ hL ha₂, rfl⟩, },
         { rw [orbit_atom_map_eq_of_mem_next_image_core_domain, next_image_core],
-          have : (((w.orbit_set_equiv (w.litter_perm.symm a.fst)).symm)
-            (inl (0, ⟨a, _⟩)) : atom).fst = w.litter_perm.symm a.fst,
-          { exact (w.orbit_set_subset _ ((w.orbit_set_equiv _).symm _).prop).1,
+          have : (((φ.orbit_set_equiv ((φ.litter_perm hφ).symm a.fst)).symm)
+            (inl (0, ⟨a, _⟩)) : atom).fst = (φ.litter_perm hφ).symm a.fst,
+          { exact (φ.orbit_set_subset _ ((φ.orbit_set_equiv _).symm _).prop).1,
             exact ⟨ha₁, ha₃⟩, },
-          rw w.orbit_set_equiv_congr _ this,
+          rw φ.orbit_set_equiv_congr _ this,
           simp only [equiv.apply_symm_apply, elim_inl, subtype.coe_eta, next_backward_image,
             subtype.coe_mk], }, }, },
     { obtain ⟨⟨b, hb₁, hb₂⟩, ha₁⟩ := ha₁,
       rw ← hb₂,
       refine ⟨b, or.inl hb₁, _⟩,
       rw orbit_atom_map_eq_of_mem_dom, },
-    { obtain ⟨a', ha'⟩ := (w.orbit_set_equiv a.fst).symm.surjective
-        ⟨a, w.mem_orbit_set_of_mem_next_image_core_domain ha₁⟩,
+    { obtain ⟨a', ha'⟩ := (φ.orbit_set_equiv a.fst).symm.surjective
+        ⟨a, φ.mem_orbit_set_of_mem_next_image_core_domain hφ ha₁⟩,
       obtain (⟨n, a'⟩ | ⟨_ | n, a'⟩) := a',
-      { have : ((w.orbit_set_equiv (w.litter_perm.symm^[n + 2] (a' : atom).fst)).symm
-          (inl (n + 1, a')) : atom) ∈ w.next_image_core_domain,
-        { refine ⟨_, ⟨w.litter_perm.symm^[n + 2] (a' : atom).fst, rfl⟩, _, ⟨_, rfl⟩, _⟩,
-          exact w.litter_perm.symm.iterate_domain (fst_mem_litter_perm_domain_of_dom a'.prop.1),
+      { have : ((φ.orbit_set_equiv ((φ.litter_perm hφ).symm^[n + 2] (a' : atom).fst)).symm
+          (inl (n + 1, a')) : atom) ∈ φ.next_image_core_domain hφ,
+        { refine ⟨_, ⟨(φ.litter_perm hφ).symm^[n + 2] (a' : atom).fst, rfl⟩, _, ⟨_, rfl⟩, _⟩,
+          exact (φ.litter_perm hφ).symm.iterate_domain
+            (fst_mem_litter_perm_domain_of_dom hφ a'.prop.1),
           refine ⟨_, _, rfl⟩,
           simp only [mem_set_of_eq, equiv.apply_symm_apply, elim_inl],
-          exact ⟨fst_mem_litter_perm_domain_of_dom a'.prop.1, rfl⟩, },
+          exact ⟨fst_mem_litter_perm_domain_of_dom hφ a'.prop.1, rfl⟩, },
         refine ⟨_, or.inr (or.inr this), _⟩,
         rw orbit_atom_map_eq_of_mem_next_image_core_domain,
         rw next_image_core,
-        have : (((w.orbit_set_equiv (w.litter_perm.symm^[n + 2] (a' : atom).fst)).symm)
-            (inl (n + 1, a')) : atom).fst = (w.litter_perm.symm^[n + 2] (a' : atom).fst) :=
-          (w.orbit_set_subset _ ((w.orbit_set_equiv _).symm _).prop).1,
-        rw w.orbit_set_equiv_congr _ this,
+        have : (((φ.orbit_set_equiv ((φ.litter_perm hφ).symm^[n + 2] (a' : atom).fst)).symm)
+            (inl (n + 1, a')) : atom).fst = ((φ.litter_perm hφ).symm^[n + 2] (a' : atom).fst) :=
+          (φ.orbit_set_subset _ ((φ.orbit_set_equiv _).symm _).prop).1,
+        rw φ.orbit_set_equiv_congr _ this,
         simp only [subtype.coe_eta, equiv.apply_symm_apply, elim_inl, next_backward_image],
         have := congr_arg subtype.val ha',
         simp only [subtype.val_eq_coe] at this,
         rw ← this,
-        refine w.orbit_set_equiv_symm_congr _,
-        have := (w.orbit_set_subset _ ((w.orbit_set_equiv _).symm _).prop).1,
+        refine φ.orbit_set_equiv_symm_congr _,
+        have := (φ.orbit_set_subset _ ((φ.orbit_set_equiv _).symm _).prop).1,
         rw mem_litter_set at this,
         rw this,
-        have := w.orbit_set_equiv_elim_of_mem_next_image_core_domain ha₁,
+        have := φ.orbit_set_equiv_elim_of_mem_next_image_core_domain hφ ha₁,
         rw ← ha' at this,
         simp only [equiv.apply_symm_apply, elim_inl, next_backward_image_domain,
           function.comp_app, mem_set_of_eq] at this,
         rw [← this.2, function.iterate_succ_apply', local_perm.right_inv],
-        exact w.litter_perm.symm.iterate_domain this.1, },
-      { have := w.orbit_set_equiv_elim_of_mem_next_image_core_domain ha₁,
+        exact (φ.litter_perm hφ).symm.iterate_domain this.1, },
+      { have := φ.orbit_set_equiv_elim_of_mem_next_image_core_domain hφ ha₁,
         rw ← ha' at this,
         simp only [equiv.apply_symm_apply, elim_inr, next_forward_image_domain,
           function.comp_app, mem_set_of_eq, function.iterate_one] at this,
         refine ⟨a', or.inr (or.inl ⟨a'.prop, this.1⟩), _⟩,
-        rw [orbit_atom_map_eq_of_need_forward_images, w.orbit_set_equiv_symm_congr this.2,
+        rw [orbit_atom_map_eq_of_need_forward_images, φ.orbit_set_equiv_symm_congr this.2,
           subtype.coe_eta, ha'],
         refl, },
-      { have : ((w.orbit_set_equiv (w.litter_perm^[n + 1] (a' : atom).fst)).symm
-          (inr (n, a')) : atom) ∈ w.next_image_core_domain,
-        { refine ⟨_, ⟨w.litter_perm^[n + 1] (a' : atom).fst, rfl⟩, _, ⟨_, rfl⟩, _⟩,
-          exact w.litter_perm.iterate_domain (fst_mem_litter_perm_domain_of_ran a'.prop.1),
+      { have : ((φ.orbit_set_equiv ((φ.litter_perm hφ)^[n + 1] (a' : atom).fst)).symm
+          (inr (n, a')) : atom) ∈ φ.next_image_core_domain hφ,
+        { refine ⟨_, ⟨(φ.litter_perm hφ)^[n + 1] (a' : atom).fst, rfl⟩, _, ⟨_, rfl⟩, _⟩,
+          exact (φ.litter_perm hφ).iterate_domain (fst_mem_litter_perm_domain_of_ran hφ a'.prop.1),
           refine ⟨_, _, rfl⟩,
           simp only [mem_set_of_eq, equiv.apply_symm_apply, elim_inl],
-          exact ⟨fst_mem_litter_perm_domain_of_ran a'.prop.1, rfl⟩, },
+          exact ⟨fst_mem_litter_perm_domain_of_ran hφ a'.prop.1, rfl⟩, },
         refine ⟨_, or.inr (or.inr this), _⟩,
         rw orbit_atom_map_eq_of_mem_next_image_core_domain,
         rw next_image_core,
-        have : (((w.orbit_set_equiv (w.litter_perm^[n + 1] (a' : atom).fst)).symm)
-            (inr (n, a')) : atom).fst = (w.litter_perm^[n + 1] (a' : atom).fst) :=
-          (w.orbit_set_subset _ ((w.orbit_set_equiv _).symm _).prop).1,
-        rw w.orbit_set_equiv_congr _ this,
+        have : (((φ.orbit_set_equiv ((φ.litter_perm hφ)^[n + 1] (a' : atom).fst)).symm)
+            (inr (n, a')) : atom).fst = ((φ.litter_perm hφ)^[n + 1] (a' : atom).fst) :=
+          (φ.orbit_set_subset _ ((φ.orbit_set_equiv _).symm _).prop).1,
+        rw φ.orbit_set_equiv_congr _ this,
         simp only [subtype.coe_eta, equiv.apply_symm_apply, elim_inl, next_backward_image],
         have := congr_arg subtype.val ha',
         simp only [subtype.val_eq_coe] at this,
         rw ← this,
-        refine w.orbit_set_equiv_symm_congr _,
-        have := (w.orbit_set_subset _ ((w.orbit_set_equiv _).symm _).prop).1,
+        refine φ.orbit_set_equiv_symm_congr _,
+        have := (φ.orbit_set_subset _ ((φ.orbit_set_equiv _).symm _).prop).1,
         rw mem_litter_set at this,
         rw this,
-        have := w.orbit_set_equiv_elim_of_mem_next_image_core_domain ha₁,
+        have := φ.orbit_set_equiv_elim_of_mem_next_image_core_domain hφ ha₁,
         rw ← ha' at this,
         simp only [equiv.apply_symm_apply, elim_inr, next_forward_image_domain,
           function.comp_app, mem_set_of_eq] at this,
@@ -902,6 +913,6 @@ begin
           function.iterate_succ_apply'], }, }, },
 end
 
-end weak_near_litter_approx
+end near_litter_action
 
 end con_nf
