src/phase2/fill_atom_range.lean
@@ -1,4 +1,4 @@
-import phase2.weak_approx
+import phase2.near_litter_action
 
 open cardinal quiver set sum with_bot
 open_locale cardinal classical pointwise
@@ -9,50 +9,50 @@ namespace con_nf
 variables [params.{u}]
 
 /-!
-# Filling in ranges of weak near-litter approximations
+# Filling in ranges of near litter actions
 TODO: Rename the gadgetry created in this file.
 -/
 
-namespace weak_near_litter_approx
+namespace near_litter_action
 
-variables (w : weak_near_litter_approx)
+variables (φ : near_litter_action)
 
 noncomputable def preimage_litter : litter :=
-w.not_banned_litter_nonempty.some
+φ.not_banned_litter_nonempty.some
 
-lemma preimage_litter_not_banned : ¬w.banned_litter w.preimage_litter :=
-w.not_banned_litter_nonempty.some.prop
+lemma preimage_litter_not_banned : ¬φ.banned_litter φ.preimage_litter :=
+φ.not_banned_litter_nonempty.some.prop
 
 /-- An atom is called *without preimage* if it is not in the range of the approximation,
 but it is in a litter near some near-litter in the range.
 Atoms without preimage need to have something map to it, so that the resulting map that we use in
 the freedom of action theorem actually maps to the correct near-litter. -/
 @[mk_iff] structure without_preimage (a : atom) : Prop :=
-(mem_map : ∃ (L : litter) (hL : (w.litter_map L).dom), a ∈ litter_set ((w.litter_map L).get hL).1)
-(not_mem_map : ∀ (L : litter) (hL : (w.litter_map L).dom), a ∉ (w.litter_map L).get hL)
-(not_mem_ran : a ∉ w.atom_map.ran)
+(mem_map : ∃ (L : litter) (hL : (φ.litter_map L).dom), a ∈ litter_set ((φ.litter_map L).get hL).1)
+(not_mem_map : ∀ (L : litter) (hL : (φ.litter_map L).dom), a ∉ (φ.litter_map L).get hL)
+(not_mem_ran : a ∉ φ.atom_map.ran)
 
 lemma without_preimage_small :
-  small {a | w.without_preimage a} :=
+  small {a | φ.without_preimage a} :=
 begin
   simp only [without_preimage_iff, set_of_and],
   rw ← inter_assoc,
   refine small.mono (inter_subset_left _ _) _,
   suffices : small ⋃ (L : litter) (hL),
-    litter_set ((w.litter_map L).get hL).1 \ (w.litter_map L).get hL,
+    litter_set ((φ.litter_map L).get hL).1 \ (φ.litter_map L).get hL,
   { refine small.mono _ this,
     rintro a ⟨⟨L, hL, ha₁⟩, ha₂⟩,
     simp only [mem_Union],
     exact ⟨L, hL, ha₁, ha₂ _ _⟩, },
   refine small.bUnion _ _,
-  { refine lt_of_le_of_lt _ w.litter_map_dom_small,
+  { refine lt_of_le_of_lt _ φ.litter_map_dom_small,
     refine ⟨⟨λ L, ⟨_, L.prop⟩, _⟩⟩,
     intros L₁ L₂ h,
     simp only [subtype.mk_eq_mk, prod.mk.inj_iff, eq_self_iff_true, and_true,
       litter.to_near_litter_injective.eq_iff, subtype.coe_inj] at h,
     exact h, },
   { intros L hL,
-    refine small.mono _ ((w.litter_map L).get hL).2.prop,
+    refine small.mono _ ((φ.litter_map L).get hL).2.prop,
     exact λ x hx, or.inl hx, },
 end
 
@@ -60,108 +60,108 @@ end
 atoms without preimage. -/
 def preimage_litter_subset : set atom :=
 (le_mk_iff_exists_subset.mp
-  (lt_of_lt_of_eq w.without_preimage_small (mk_litter_set w.preimage_litter).symm).le).some
+  (lt_of_lt_of_eq φ.without_preimage_small (mk_litter_set φ.preimage_litter).symm).le).some
 
 lemma preimage_litter_subset_spec :
-  w.preimage_litter_subset ⊆ litter_set w.preimage_litter ∧
-    #w.preimage_litter_subset = #{a : atom | w.without_preimage a} :=
+  φ.preimage_litter_subset ⊆ litter_set φ.preimage_litter ∧
+    #φ.preimage_litter_subset = #{a : atom | φ.without_preimage a} :=
 (le_mk_iff_exists_subset.mp
-  (lt_of_lt_of_eq w.without_preimage_small (mk_litter_set w.preimage_litter).symm).le).some_spec
+  (lt_of_lt_of_eq φ.without_preimage_small (mk_litter_set φ.preimage_litter).symm).le).some_spec
 
 lemma preimage_litter_subset_subset :
-  w.preimage_litter_subset ⊆ litter_set w.preimage_litter :=
-w.preimage_litter_subset_spec.1
+  φ.preimage_litter_subset ⊆ litter_set φ.preimage_litter :=
+φ.preimage_litter_subset_spec.1
 
 lemma preimage_litter_subset_small :
-  small (w.preimage_litter_subset) :=
-lt_of_eq_of_lt w.preimage_litter_subset_spec.2 w.without_preimage_small
+  small (φ.preimage_litter_subset) :=
+lt_of_eq_of_lt φ.preimage_litter_subset_spec.2 φ.without_preimage_small
 
 @[irreducible] noncomputable def preimage_litter_equiv :
-  w.preimage_litter_subset ≃ {a : atom | w.without_preimage a} :=
-(cardinal.eq.mp w.preimage_litter_subset_spec.2).some
+  φ.preimage_litter_subset ≃ {a : atom | φ.without_preimage a} :=
+(cardinal.eq.mp φ.preimage_litter_subset_spec.2).some
 
 /-- The images of atoms in a litter `L` that were mapped outside the target litter, but
 were not in the domain. -/
-@[mk_iff] structure mapped_outside (L : litter) (hL : (w.litter_map L).dom) (a : atom) : Prop :=
-(mem_map : a ∈ (w.litter_map L).get hL)
-(not_mem_map : a ∉ litter_set ((w.litter_map L).get hL).1)
-(not_mem_ran : a ∉ w.atom_map.ran)
+@[mk_iff] structure mapped_outside (L : litter) (hL : (φ.litter_map L).dom) (a : atom) : Prop :=
+(mem_map : a ∈ (φ.litter_map L).get hL)
+(not_mem_map : a ∉ litter_set ((φ.litter_map L).get hL).1)
+(not_mem_ran : a ∉ φ.atom_map.ran)
 
 /-- There are only `< κ`-many atoms in a litter `L` that are mapped outside the image litter,
 and that are not already in the domain. -/
-lemma mapped_outside_small (L : litter) (hL : (w.litter_map L).dom) :
-  small {a | w.mapped_outside L hL a} :=
+lemma mapped_outside_small (L : litter) (hL : (φ.litter_map L).dom) :
+  small {a | φ.mapped_outside L hL a} :=
 begin
   simp only [mapped_outside_iff, set_of_and],
   rw ← inter_assoc,
   refine small.mono (inter_subset_left _ _) _,
-  refine small.mono _ ((w.litter_map L).get hL).2.prop,
+  refine small.mono _ ((φ.litter_map L).get hL).2.prop,
   exact λ x hx, or.inr hx,
 end
 
-lemma without_preimage.not_mapped_outside {a : atom} (ha : w.without_preimage a)
-  (L : litter) (hL : (w.litter_map L).dom) : ¬w.mapped_outside L hL a :=
+lemma without_preimage.not_mapped_outside {a : atom} (ha : φ.without_preimage a)
+  (L : litter) (hL : (φ.litter_map L).dom) : ¬φ.mapped_outside L hL a :=
 λ ha', ha.not_mem_map L hL ha'.mem_map
 
-lemma mapped_outside.not_without_preimage {a : atom} {L : litter} {hL : (w.litter_map L).dom}
-  (ha : w.mapped_outside L hL a) : ¬w.without_preimage a :=
+lemma mapped_outside.not_without_preimage {a : atom} {L : litter} {hL : (φ.litter_map L).dom}
+  (ha : φ.mapped_outside L hL a) : ¬φ.without_preimage a :=
 λ ha', ha'.not_mem_map L hL ha.mem_map
 
 /-- The amount of atoms in a litter that are not in the domain already is `κ`. -/
-lemma mk_mapped_outside_domain (L : litter) : #(litter_set L \ w.atom_map.dom : set atom) = #κ :=
+lemma mk_mapped_outside_domain (L : litter) : #(litter_set L \ φ.atom_map.dom : set atom) = #κ :=
 begin
   refine le_antisymm _ _,
   { rw ← mk_litter_set,
     exact mk_subtype_mono (λ x hx, hx.1), },
   by_contra' h,
-  have := small.union h w.atom_map_dom_small,
+  have := small.union h φ.atom_map_dom_small,
   rw diff_union_self at this,
   exact (mk_litter_set L).not_lt (small.mono (subset_union_left _ _) this),
 end
 
 /-- To each litter we associate a subset which is to contain the atoms mapped outside it. -/
-def mapped_outside_subset (L : litter) (hL : (w.litter_map L).dom) : set atom :=
+def mapped_outside_subset (L : litter) (hL : (φ.litter_map L).dom) : set atom :=
 (le_mk_iff_exists_subset.mp
-  (lt_of_lt_of_eq (w.mapped_outside_small L hL) (w.mk_mapped_outside_domain L).symm).le).some
+  (lt_of_lt_of_eq (φ.mapped_outside_small L hL) (φ.mk_mapped_outside_domain L).symm).le).some
 
-lemma mapped_outside_subset_spec (L : litter) (hL : (w.litter_map L).dom) :
-  w.mapped_outside_subset L hL ⊆ litter_set L \ w.atom_map.dom ∧
-    #(w.mapped_outside_subset L hL) = #{a : atom | w.mapped_outside L hL a} :=
+lemma mapped_outside_subset_spec (L : litter) (hL : (φ.litter_map L).dom) :
+  φ.mapped_outside_subset L hL ⊆ litter_set L \ φ.atom_map.dom ∧
+    #(φ.mapped_outside_subset L hL) = #{a : atom | φ.mapped_outside L hL a} :=
 (le_mk_iff_exists_subset.mp
-  (lt_of_lt_of_eq (w.mapped_outside_small L hL) (w.mk_mapped_outside_domain L).symm).le).some_spec
+  (lt_of_lt_of_eq (φ.mapped_outside_small L hL) (φ.mk_mapped_outside_domain L).symm).le).some_spec
 
-lemma mapped_outside_subset_subset (L : litter) (hL : (w.litter_map L).dom) :
-  w.mapped_outside_subset L hL ⊆ litter_set L :=
-λ x hx, ((w.mapped_outside_subset_spec L hL).1 hx).1
+lemma mapped_outside_subset_subset (L : litter) (hL : (φ.litter_map L).dom) :
+  φ.mapped_outside_subset L hL ⊆ litter_set L :=
+λ x hx, ((φ.mapped_outside_subset_spec L hL).1 hx).1
 
-lemma mapped_outside_subset_closure (L : litter) (hL : (w.litter_map L).dom) :
-  w.mapped_outside_subset L hL ⊆ w.atom_map.domᶜ :=
-λ x hx, ((w.mapped_outside_subset_spec L hL).1 hx).2
+lemma mapped_outside_subset_closure (L : litter) (hL : (φ.litter_map L).dom) :
+  φ.mapped_outside_subset L hL ⊆ φ.atom_map.domᶜ :=
+λ x hx, ((φ.mapped_outside_subset_spec L hL).1 hx).2
 
-lemma mapped_outside_subset_small (L : litter) (hL : (w.litter_map L).dom) :
-  small (w.mapped_outside_subset L hL) :=
-lt_of_eq_of_lt (w.mapped_outside_subset_spec L hL).2 (w.mapped_outside_small L hL)
+lemma mapped_outside_subset_small (L : litter) (hL : (φ.litter_map L).dom) :
+  small (φ.mapped_outside_subset L hL) :=
+lt_of_eq_of_lt (φ.mapped_outside_subset_spec L hL).2 (φ.mapped_outside_small L hL)
 
 /-- A correspondence between the "mapped outside" subset of `L` and its atoms which were mapped
 outside the target litter. We will use this equivalence to construct an approximation to
 use in the freedom of action theorem. -/
-@[irreducible] noncomputable def mapped_outside_equiv (L : litter) (hL : (w.litter_map L).dom) :
-  w.mapped_outside_subset L hL ≃ {a : atom | w.mapped_outside L hL a} :=
-(cardinal.eq.mp (w.mapped_outside_subset_spec L hL).2).some
+@[irreducible] noncomputable def mapped_outside_equiv (L : litter) (hL : (φ.litter_map L).dom) :
+  φ.mapped_outside_subset L hL ≃ {a : atom | φ.mapped_outside L hL a} :=
+(cardinal.eq.mp (φ.mapped_outside_subset_spec L hL).2).some
 
 noncomputable def supported_action_atom_map_core : atom →. atom :=
 λ a, {
-  dom := (w.atom_map a).dom ∨ a ∈ w.preimage_litter_subset ∨
-    ∃ L hL, a ∈ w.mapped_outside_subset L hL,
-  get := λ h, h.elim' (w.atom_map a).get
+  dom := (φ.atom_map a).dom ∨ a ∈ φ.preimage_litter_subset ∨
+    ∃ L hL, a ∈ φ.mapped_outside_subset L hL,
+  get := λ h, h.elim' (φ.atom_map a).get
     (λ h, h.elim'
-      (λ h, w.preimage_litter_equiv ⟨a, h⟩)
-      (λ h, w.mapped_outside_equiv h.some h.some_spec.some ⟨a, h.some_spec.some_spec⟩)),
+      (λ h, φ.preimage_litter_equiv ⟨a, h⟩)
+      (λ h, φ.mapped_outside_equiv h.some h.some_spec.some ⟨a, h.some_spec.some_spec⟩)),
 }
 
 lemma mem_supported_action_atom_map_core_dom_iff (a : atom) :
-  (w.supported_action_atom_map_core a).dom ↔
-  a ∈ w.atom_map.dom ∪ w.preimage_litter_subset ∪ ⋃ L hL, w.mapped_outside_subset L hL :=
+  (φ.supported_action_atom_map_core a).dom ↔
+  a ∈ φ.atom_map.dom ∪ φ.preimage_litter_subset ∪ ⋃ L hL, φ.mapped_outside_subset L hL :=
 begin
   rw supported_action_atom_map_core,
   simp only [pfun.dom_mk, mem_set_of_eq, mem_union, mem_Union],
@@ -170,97 +170,97 @@ begin
 end
 
 lemma supported_action_atom_map_core_dom_eq :
-  w.supported_action_atom_map_core.dom =
-  w.atom_map.dom ∪ w.preimage_litter_subset ∪ ⋃ L hL, w.mapped_outside_subset L hL :=
+  φ.supported_action_atom_map_core.dom =
+  φ.atom_map.dom ∪ φ.preimage_litter_subset ∪ ⋃ L hL, φ.mapped_outside_subset L hL :=
 begin
   ext a : 1,
-  exact w.mem_supported_action_atom_map_core_dom_iff a,
+  exact φ.mem_supported_action_atom_map_core_dom_iff a,
 end
 
 lemma supported_action_atom_map_core_dom_small :
-  small w.supported_action_atom_map_core.dom :=
+  small φ.supported_action_atom_map_core.dom :=
 begin
   rw supported_action_atom_map_core_dom_eq,
-  refine small.union (small.union w.atom_map_dom_small _) _,
-  { exact w.preimage_litter_subset_small, },
+  refine small.union (small.union φ.atom_map_dom_small _) _,
+  { exact φ.preimage_litter_subset_small, },
   { refine small.bUnion _ _,
-    { refine lt_of_le_of_lt _ w.litter_map_dom_small,
+    { refine lt_of_le_of_lt _ φ.litter_map_dom_small,
       refine ⟨⟨λ L, ⟨_, L.prop⟩, λ L₁ L₂ h, _⟩⟩,
       simp only [subtype.mk_eq_mk, prod.mk.inj_iff, eq_self_iff_true, and_true,
         litter.to_near_litter_injective.eq_iff, subtype.coe_inj] at h,
       exact h, },
     { intros L hL,
-      exact w.mapped_outside_subset_small L hL, }, },
+      exact φ.mapped_outside_subset_small L hL, }, },
 end
 
 lemma mk_supported_action_atom_map_dom :
-  #(w.supported_action_atom_map_core.dom ∆
-    ((λ a, part.get_or_else (w.supported_action_atom_map_core a) (arbitrary atom)) ''
-      w.supported_action_atom_map_core.dom) : set atom) ≤
-  #(litter_set $ w.preimage_litter) :=
+  #(φ.supported_action_atom_map_core.dom ∆
+    ((λ a, part.get_or_else (φ.supported_action_atom_map_core a) (arbitrary atom)) ''
+      φ.supported_action_atom_map_core.dom) : set atom) ≤
+  #(litter_set $ φ.preimage_litter) :=
 begin
   rw mk_litter_set,
   refine le_trans (mk_subtype_mono symm_diff_subset_union) (le_trans (mk_union_le _ _) _),
   refine add_le_of_le κ_regular.aleph_0_le _ _,
-  exact le_of_lt w.supported_action_atom_map_core_dom_small,
-  exact le_trans mk_image_le (le_of_lt w.supported_action_atom_map_core_dom_small),
+  exact le_of_lt φ.supported_action_atom_map_core_dom_small,
+  exact le_trans mk_image_le (le_of_lt φ.supported_action_atom_map_core_dom_small),
 end
 
-lemma supported_action_eq_of_dom {a : atom} (ha : (w.atom_map a).dom) :
-  (w.supported_action_atom_map_core a).get (or.inl ha) = (w.atom_map a).get ha :=
+lemma supported_action_eq_of_dom {a : atom} (ha : (φ.atom_map a).dom) :
+  (φ.supported_action_atom_map_core a).get (or.inl ha) = (φ.atom_map a).get ha :=
 begin
   simp only [supported_action_atom_map_core],
   rw or.elim'_left,
 end
 
 lemma supported_action_eq_of_mem_preimage_litter_subset {a : atom}
-  (ha : a ∈ w.preimage_litter_subset) :
-  (w.supported_action_atom_map_core a).get (or.inr (or.inl ha)) = w.preimage_litter_equiv ⟨a, ha⟩ :=
+  (ha : a ∈ φ.preimage_litter_subset) :
+  (φ.supported_action_atom_map_core a).get (or.inr (or.inl ha)) = φ.preimage_litter_equiv ⟨a, ha⟩ :=
 begin
   simp only [supported_action_atom_map_core],
   rw [or.elim'_right, or.elim'_left],
   intro h',
-  have := w.preimage_litter_not_banned,
+  have := φ.preimage_litter_not_banned,
   rw banned_litter_iff at this,
   push_neg at this,
-  exact this.1 a h' (w.preimage_litter_subset_subset ha).symm,
+  exact this.1 a h' (φ.preimage_litter_subset_subset ha).symm,
 end
 
 lemma supported_action_eq_of_mem_mapped_outside_subset {a : atom}
-  {L hL} (ha : a ∈ w.mapped_outside_subset L hL) :
-  (w.supported_action_atom_map_core a).get (or.inr (or.inr ⟨L, hL, ha⟩)) =
-  w.mapped_outside_equiv L hL ⟨a, ha⟩ :=
+  {L hL} (ha : a ∈ φ.mapped_outside_subset L hL) :
+  (φ.supported_action_atom_map_core a).get (or.inr (or.inr ⟨L, hL, ha⟩)) =
+  φ.mapped_outside_equiv L hL ⟨a, ha⟩ :=
 begin
-  have : ∃ L hL, a ∈ w.mapped_outside_subset L hL := ⟨L, hL, ha⟩,
+  have : ∃ L hL, a ∈ φ.mapped_outside_subset L hL := ⟨L, hL, ha⟩,
   simp only [supported_action_atom_map_core],
   rw [or.elim'_right, or.elim'_right],
   { cases eq_of_mem_litter_set_of_mem_litter_set
-      (w.mapped_outside_subset_subset _ hL ha)
-      (w.mapped_outside_subset_subset _ this.some_spec.some this.some_spec.some_spec),
+      (φ.mapped_outside_subset_subset _ hL ha)
+      (φ.mapped_outside_subset_subset _ this.some_spec.some this.some_spec.some_spec),
     refl, },
   { intro h,
     have := eq_of_mem_litter_set_of_mem_litter_set
-      (w.mapped_outside_subset_subset _ hL ha)
-      (w.preimage_litter_subset_subset h),
+      (φ.mapped_outside_subset_subset _ hL ha)
+      (φ.preimage_litter_subset_subset h),
     cases this,
-    have := w.preimage_litter_not_banned,
+    have := φ.preimage_litter_not_banned,
     rw banned_litter_iff at this,
     push_neg at this,
     cases this.2.1 hL, },
   { exact ((mapped_outside_subset_spec _ _ hL).1 ha).2, },
 end
 
-lemma supported_action_atom_map_core_injective ⦃a b : atom⦄
-  (ha :  (supported_action_atom_map_core w a).dom) (hb :  (supported_action_atom_map_core w b).dom)
-  (hab : (w.supported_action_atom_map_core a).get ha =
-    (w.supported_action_atom_map_core b).get hb) :
+lemma supported_action_atom_map_core_injective ⦃a b : atom⦄ (hφ : φ.lawful)
+  (ha : (supported_action_atom_map_core φ a).dom) (hb : (supported_action_atom_map_core φ b).dom)
+  (hab : (φ.supported_action_atom_map_core a).get ha =
+    (φ.supported_action_atom_map_core b).get hb) :
   a = b :=
 begin
   obtain (ha | ha | ⟨L, hL, ha⟩) := ha;
   obtain (hb | hb | ⟨L', hL', hb⟩) := hb,
   { have := (supported_action_eq_of_dom _ ha).symm.trans
       (hab.trans (supported_action_eq_of_dom _ hb)),
-    exact w.atom_map_injective ha hb this, },
+    exact hφ.atom_map_injective ha hb this, },
   { have := (supported_action_eq_of_dom _ ha).symm.trans
       (hab.trans (supported_action_eq_of_mem_preimage_litter_subset _ hb)),
     obtain ⟨hab, -⟩ := subtype.coe_eq_iff.mp this.symm,
@@ -280,8 +280,8 @@ begin
   { have := (supported_action_eq_of_mem_preimage_litter_subset _ ha).symm.trans
       (hab.trans (supported_action_eq_of_mem_mapped_outside_subset _ hb)),
     obtain ⟨hab, -⟩ := subtype.coe_eq_iff.mp this,
-    cases without_preimage.not_mapped_outside w hab _ hL'
-      (w.mapped_outside_equiv L' hL' ⟨b, hb⟩).prop, },
+    cases without_preimage.not_mapped_outside φ hab _ hL'
+      (φ.mapped_outside_equiv L' hL' ⟨b, hb⟩).prop, },
   { have := (supported_action_eq_of_mem_mapped_outside_subset _ ha).symm.trans
       (hab.trans (supported_action_eq_of_dom _ hb)),
     obtain ⟨hab, -⟩ := subtype.coe_eq_iff.mp this,
@@ -289,110 +289,114 @@ begin
   { have := (supported_action_eq_of_mem_mapped_outside_subset _ ha).symm.trans
       (hab.trans (supported_action_eq_of_mem_preimage_litter_subset _ hb)),
     obtain ⟨hab, -⟩ := subtype.coe_eq_iff.mp this.symm,
-    cases without_preimage.not_mapped_outside w hab _ hL
-      (w.mapped_outside_equiv L hL ⟨a, ha⟩).prop, },
+    cases without_preimage.not_mapped_outside φ hab _ hL
+      (φ.mapped_outside_equiv L hL ⟨a, ha⟩).prop, },
   { have := (supported_action_eq_of_mem_mapped_outside_subset _ ha).symm.trans
       (hab.trans (supported_action_eq_of_mem_mapped_outside_subset _ hb)),
-    cases w.litter_map_injective hL hL' _,
+    cases hφ.litter_map_injective hL hL' _,
     { simp only [subtype.coe_inj, embedding_like.apply_eq_iff_eq] at this,
       exact this, },
     obtain ⟨hab, -⟩ := subtype.coe_eq_iff.mp this,
-    exact ⟨_, hab.1, (w.mapped_outside_equiv L' hL' ⟨b, hb⟩).prop.1⟩, },
+    exact ⟨_, hab.1, (φ.mapped_outside_equiv L' hL' ⟨b, hb⟩).prop.1⟩, },
 end
 
-lemma supported_action_atom_map_core_mem (a : atom) (ha : (w.supported_action_atom_map_core a).dom)
-  (L : litter) (hL : (w.litter_map L).dom) :
-  a.fst = L ↔ (w.supported_action_atom_map_core a).get ha ∈ (w.litter_map L).get hL :=
+lemma supported_action_atom_map_core_mem (hφ : φ.lawful)
+  (a : atom) (ha : (φ.supported_action_atom_map_core a).dom)
+  (L : litter) (hL : (φ.litter_map L).dom) :
+  a.fst = L ↔ (φ.supported_action_atom_map_core a).get ha ∈ (φ.litter_map L).get hL :=
 begin
   obtain (ha | ha | ⟨L', hL', ha⟩) := ha,
-  { rw [w.atom_mem a ha L hL, supported_action_eq_of_dom], },
+  { rw [hφ.atom_mem a ha L hL, supported_action_eq_of_dom], },
   { rw supported_action_eq_of_mem_preimage_litter_subset,
     split,
     { rintro rfl,
-      have := w.preimage_litter_subset_subset ha,
+      have := φ.preimage_litter_subset_subset ha,
       rw mem_litter_set at this,
       rw this at hL,
       have := banned_litter.litter_dom _ hL,
-      cases w.preimage_litter_not_banned this, },
+      cases φ.preimage_litter_not_banned this, },
     { intro h,
-      cases (w.preimage_litter_equiv ⟨a, ha⟩).prop.not_mem_map L hL h, }, },
-  { cases w.mapped_outside_subset_subset L' hL' ha,
+      cases (φ.preimage_litter_equiv ⟨a, ha⟩).prop.not_mem_map L hL h, }, },
+  { cases φ.mapped_outside_subset_subset L' hL' ha,
     rw supported_action_eq_of_mem_mapped_outside_subset,
     split,
     { rintro rfl,
-      exact (w.mapped_outside_equiv _ _ _ ).prop.mem_map, },
+      exact (φ.mapped_outside_equiv _ _ _ ).prop.mem_map, },
     { intro h,
-      refine w.litter_map_injective hL' hL ⟨_, _, h⟩,
-      exact (w.mapped_outside_equiv _ _ _ ).prop.mem_map, }, },
+      refine hφ.litter_map_injective hL' hL ⟨_, _, h⟩,
+      exact (φ.mapped_outside_equiv _ _ _ ).prop.mem_map, }, },
 end
 
-noncomputable def fill_atom_range : weak_near_litter_approx := {
-  atom_map := w.supported_action_atom_map_core,
-  litter_map := w.litter_map,
-  atom_map_dom_small := w.supported_action_atom_map_core_dom_small,
-  litter_map_dom_small := w.litter_map_dom_small,
-  atom_map_injective := w.supported_action_atom_map_core_injective,
-  litter_map_injective := w.litter_map_injective,
-  atom_mem := w.supported_action_atom_map_core_mem,
+noncomputable def fill_atom_range : near_litter_action := {
+  atom_map := φ.supported_action_atom_map_core,
+  litter_map := φ.litter_map,
+  atom_map_dom_small := φ.supported_action_atom_map_core_dom_small,
+  litter_map_dom_small := φ.litter_map_dom_small,
 }
 
-variable {w}
+lemma fill_atom_range_lawful (hφ : φ.lawful) : φ.fill_atom_range.lawful := {
+  atom_map_injective := λ a b, φ.supported_action_atom_map_core_injective hφ,
+  litter_map_injective := hφ.litter_map_injective,
+  atom_mem := φ.supported_action_atom_map_core_mem hφ,
+}
+
+variable {φ}
 
 @[simp] lemma fill_atom_range_atom_map :
-  w.fill_atom_range.atom_map = w.supported_action_atom_map_core := rfl
+  φ.fill_atom_range.atom_map = φ.supported_action_atom_map_core := rfl
 
 @[simp] lemma fill_atom_range_litter_map :
-  w.fill_atom_range.litter_map = w.litter_map := rfl
+  φ.fill_atom_range.litter_map = φ.litter_map := rfl
 
 lemma subset_supported_action_atom_map_core_dom :
-  w.atom_map.dom ⊆ w.supported_action_atom_map_core.dom :=
+  φ.atom_map.dom ⊆ φ.supported_action_atom_map_core.dom :=
 subset_union_left _ _
 
 lemma subset_supported_action_atom_map_core_ran :
-  w.atom_map.ran ⊆ w.supported_action_atom_map_core.ran :=
+  φ.atom_map.ran ⊆ φ.supported_action_atom_map_core.ran :=
 begin
   rintro _ ⟨a, ha, rfl⟩,
-  exact ⟨a, subset_supported_action_atom_map_core_dom ha, w.supported_action_eq_of_dom _⟩,
+  exact ⟨a, subset_supported_action_atom_map_core_dom ha, φ.supported_action_eq_of_dom _⟩,
 end
 
-lemma fill_atom_range_symm_diff_subset_ran
-  (L : litter) (hL : (w.fill_atom_range.litter_map L).dom) :
-  ((w.fill_atom_range.litter_map L).get hL : set atom) ∆ litter_set
-    ((w.fill_atom_range.litter_map L).get hL).fst ⊆ w.fill_atom_range.atom_map.ran :=
+lemma fill_atom_range_symm_diff_subset_ran (hφ : φ.lawful)
+  (L : litter) (hL : (φ.fill_atom_range.litter_map L).dom) :
+  ((φ.fill_atom_range.litter_map L).get hL : set atom) ∆ litter_set
+    ((φ.fill_atom_range.litter_map L).get hL).fst ⊆ φ.fill_atom_range.atom_map.ran :=
 begin
   rintro a,
-  by_cases ha₁ : a ∈ w.atom_map.ran,
+  by_cases ha₁ : a ∈ φ.atom_map.ran,
   { obtain ⟨b, hb, rfl⟩ := ha₁,
-    exact λ _, ⟨b, or.inl hb, w.supported_action_eq_of_dom hb⟩, },
+    exact λ _, ⟨b, or.inl hb, φ.supported_action_eq_of_dom hb⟩, },
   rintro (⟨ha₂, ha₃⟩ | ⟨ha₂, ha₃⟩),
-  { refine ⟨(w.mapped_outside_equiv L hL).symm ⟨a, ha₂, ha₃, ha₁⟩, _, _⟩,
-    { exact or.inr (or.inr ⟨L, hL, ((w.mapped_outside_equiv L hL).symm _).prop⟩), },
+  { refine ⟨(φ.mapped_outside_equiv L hL).symm ⟨a, ha₂, ha₃, ha₁⟩, _, _⟩,
+    { exact or.inr (or.inr ⟨L, hL, ((φ.mapped_outside_equiv L hL).symm _).prop⟩), },
     { simp only [fill_atom_range_atom_map],
-      refine (w.supported_action_eq_of_mem_mapped_outside_subset
-        ((w.mapped_outside_equiv L hL).symm _).prop).trans _,
+      refine (φ.supported_action_eq_of_mem_mapped_outside_subset
+        ((φ.mapped_outside_equiv L hL).symm _).prop).trans _,
       simp only [subtype.coe_eta, equiv.apply_symm_apply, subtype.coe_mk], }, },
-  { by_cases ha₄ : ∀ (L' : litter) (hL' : (w.litter_map L').dom), a ∉ (w.litter_map L').get hL',
-    { refine ⟨w.preimage_litter_equiv.symm ⟨a, ⟨L, hL, ha₂⟩, ha₄, ha₁⟩, _, _⟩,
-      { exact or.inr (or.inl (w.preimage_litter_equiv.symm _).prop), },
+  { by_cases ha₄ : ∀ (L' : litter) (hL' : (φ.litter_map L').dom), a ∉ (φ.litter_map L').get hL',
+    { refine ⟨φ.preimage_litter_equiv.symm ⟨a, ⟨L, hL, ha₂⟩, ha₄, ha₁⟩, _, _⟩,
+      { exact or.inr (or.inl (φ.preimage_litter_equiv.symm _).prop), },
       { simp only [fill_atom_range_atom_map],
-        refine (w.supported_action_eq_of_mem_preimage_litter_subset
-          (w.preimage_litter_equiv.symm _).prop).trans _,
+        refine (φ.supported_action_eq_of_mem_preimage_litter_subset
+          (φ.preimage_litter_equiv.symm _).prop).trans _,
         simp only [subtype.coe_eta, equiv.apply_symm_apply, subtype.coe_mk], }, },
     { push_neg at ha₄,
       obtain ⟨L', hL', ha₄⟩ := ha₄,
-      refine ⟨(w.mapped_outside_equiv L' hL').symm ⟨a, ha₄, _, ha₁⟩, _, _⟩,
+      refine ⟨(φ.mapped_outside_equiv L' hL').symm ⟨a, ha₄, _, ha₁⟩, _, _⟩,
       { intro ha,
         have := near_litter.inter_nonempty_of_fst_eq_fst
           (eq_of_mem_litter_set_of_mem_litter_set ha₂ ha),
-        cases w.litter_map_injective hL hL' this,
+        cases hφ.litter_map_injective hL hL' this,
         exact ha₃ ha₄, },
-      { exact or.inr (or.inr ⟨L', hL', ((w.mapped_outside_equiv L' hL').symm _).prop⟩), },
+      { exact or.inr (or.inr ⟨L', hL', ((φ.mapped_outside_equiv L' hL').symm _).prop⟩), },
       { simp only [fill_atom_range_atom_map],
-        refine (w.supported_action_eq_of_mem_mapped_outside_subset
-          ((w.mapped_outside_equiv L' hL').symm _).prop).trans _,
+        refine (φ.supported_action_eq_of_mem_mapped_outside_subset
+          ((φ.mapped_outside_equiv L' hL').symm _).prop).trans _,
         simp only [subtype.coe_eta, equiv.apply_symm_apply, subtype.coe_mk], }, }, },
 end
 
-end weak_near_litter_approx
+end near_litter_action
 
 end con_nf
