src/phase2/refine.lean
@@ -1,3 +1,4 @@
+import phase2.struct_action
 import phase2.fill_atom_range
 import phase2.fill_atom_orbits
 
@@ -7,20 +8,20 @@ namespace con_nf
 variables [params.{u}]
 
 /-!
-# Refinements of weak approximations
+# Refinements of actions
 -/
 
-namespace weak_near_litter_approx
+namespace near_litter_action
 
-variables (w : weak_near_litter_approx)
+variables (φ : near_litter_action) (hφ : φ.lawful)
 
-noncomputable def refine : weak_near_litter_approx :=
-w.fill_atom_range.fill_atom_orbits fill_atom_range_symm_diff_subset_ran
+noncomputable def refine (hφ : φ.lawful) : near_litter_action :=
+φ.fill_atom_range.fill_atom_orbits (φ.fill_atom_range_lawful hφ)
 
-variable {w}
+variables {φ} {hφ}
 
-@[simp] lemma refine_atom_map {a : atom} (ha : (w.atom_map a).dom) :
-  w.refine.atom_map a = w.atom_map a :=
+@[simp] lemma refine_atom_map {a : atom} (ha : (φ.atom_map a).dom) :
+  (φ.refine hφ).atom_map a = φ.atom_map a :=
 begin
   unfold refine,
   refine part.ext' _ _,
@@ -28,43 +29,44 @@ begin
       iff_true],
     exact or.inl (or.inl ha), },
   intros h₁ h₂,
-  refine (w.fill_atom_range.orbit_atom_map_eq_of_mem_dom _ (or.inl ha)).trans _,
-  exact w.supported_action_eq_of_dom ha,
+  refine (φ.fill_atom_range.orbit_atom_map_eq_of_mem_dom _ _ (or.inl ha)).trans _,
+  exact φ.supported_action_eq_of_dom ha,
 end
 
-@[simp] lemma refine_atom_map_get {a : atom} (ha : (w.atom_map a).dom) :
-  (w.refine.atom_map a).get (or.inl (or.inl ha)) = (w.atom_map a).get ha :=
+@[simp] lemma refine_atom_map_get {a : atom} (ha : (φ.atom_map a).dom) :
+  ((φ.refine hφ).atom_map a).get (or.inl (or.inl ha)) = (φ.atom_map a).get ha :=
 by simp only [refine_atom_map ha]
 
-@[simp] lemma refine_litter_map : w.refine.litter_map = w.litter_map := rfl
+@[simp] lemma refine_litter_map : (φ.refine hφ).litter_map = φ.litter_map := rfl
 
-lemma refine_precise : precise w.refine :=
-fill_atom_orbits_precise fill_atom_range_symm_diff_subset_ran
+lemma refine_precise : precise (φ.refine hφ) :=
+fill_atom_orbits_precise _ (fill_atom_range_symm_diff_subset_ran hφ)
 
-end weak_near_litter_approx
+end near_litter_action
 
-namespace weak_struct_approx
+namespace struct_action
 
-variables {β : type_index} (w : weak_struct_approx β)
+variables {β : type_index} (φ : struct_action β) (hφ : φ.lawful)
 
-noncomputable def refine : weak_struct_approx β := λ A, (w A).refine
+noncomputable def refine : struct_action β := λ A, (φ A).refine (hφ A)
 
 @[simp] lemma refine_apply {A : extended_index β} :
-  w.refine A = (w A).refine := rfl
+  φ.refine hφ A = (φ A).refine (hφ A) := rfl
 
-@[simp] lemma refine_atom_map {A : extended_index β} {a : atom} (ha : ((w A).atom_map a).dom) :
-  (w A).refine.atom_map a = (w A).atom_map a := weak_near_litter_approx.refine_atom_map ha
+@[simp] lemma refine_atom_map {A : extended_index β} {a : atom} (ha : ((φ A).atom_map a).dom) :
+  ((φ A).refine (hφ A)).atom_map a = (φ A).atom_map a := near_litter_action.refine_atom_map ha
 
-@[simp] lemma refine_atom_map_get {A : extended_index β} {a : atom} (ha : ((w A).atom_map a).dom) :
-  ((w A).refine.atom_map a).get (or.inl (or.inl ha)) = ((w A).atom_map a).get ha :=
-weak_near_litter_approx.refine_atom_map_get ha
+-- TODO: check confluence with previous lemma
+@[simp] lemma refine_atom_map_get {A : extended_index β} {a : atom} (ha : ((φ A).atom_map a).dom) :
+  (((φ A).refine (hφ A)).atom_map a).get (or.inl (or.inl ha)) = ((φ A).atom_map a).get ha :=
+near_litter_action.refine_atom_map_get ha
 
 @[simp] lemma refine_litter_map {A : extended_index β} :
-  (w A).refine.litter_map = (w A).litter_map := rfl
+  ((φ A).refine (hφ A)).litter_map = (φ A).litter_map := rfl
 
-lemma refine_precise : precise w.refine :=
-λ A, weak_near_litter_approx.refine_precise
+lemma refine_precise : precise (φ.refine hφ) :=
+λ A, near_litter_action.refine_precise
 
-end weak_struct_approx
+end struct_action
 
 end con_nf
