src/phase2/struct_action.lean
@@ -1,0 +1,270 @@
+import phase2.near_litter_action
+
+open cardinal quiver set sum with_bot
+open_locale cardinal classical pointwise
+
+universe u
+
+namespace con_nf
+variable [params.{u}]
+
+/-!
+# Structural actions
+-/
+
+/-- A `β`-structural action is a product that assigns a near-litter action to each `β`-extended
+index. -/
+def struct_action (β : type_index) := extended_index β → near_litter_action
+
+def struct_action.lawful {β : type_index} (φ : struct_action β) : Prop := ∀ B, (φ B).lawful
+
+namespace struct_action
+
+section precise
+
+def precise {β : type_index} (φ : struct_action β) : Prop :=
+∀ B, (φ B).precise
+
+variables {α : Λ} [position_data.{}] [phase_2_assumptions α] {β : Iio α} (φ : struct_action β)
+
+noncomputable def complete (hφ : φ.lawful) : struct_approx β :=
+λ B, (φ B).complete (hφ B) B
+
+lemma smul_atom_eq {hφ : φ.lawful}
+  {π : struct_perm β} (hπ : (φ.complete hφ).exactly_approximates π)
+  {a : atom} {B : extended_index β} (ha : ((φ B).atom_map a).dom) :
+  struct_perm.derivative B π • a = ((φ B).atom_map a).get ha :=
+begin
+  have := (φ B).smul_atom_eq (hπ B) ha,
+  rw struct_perm.of_bot_smul at this,
+  exact this,
+end
+
+lemma smul_to_near_litter_eq_of_precise {hφ : φ.lawful} (hφp : φ.precise)
+  {π : struct_perm β} (hπ : (φ.complete hφ).exactly_approximates π)
+  {L : litter} {B : extended_index β} (hL : ((φ B).litter_map L).dom)
+  (hπL : struct_perm.derivative B π • L = (((φ B).litter_map L).get hL).1) :
+  struct_perm.derivative B π • L.to_near_litter = ((φ B).litter_map L).get hL :=
+begin
+  have := (φ B).smul_to_near_litter_eq_of_precise_at (hπ B) hL (hφp B hL) _,
+  { rw struct_perm.of_bot_smul at this,
+    exact this, },
+  { rw struct_perm.of_bot_smul,
+    exact hπL, },
+end
+
+lemma smul_near_litter_eq_of_precise {hφ : φ.lawful} (hφp : φ.precise)
+  {π : struct_perm β} (hπ : (φ.complete hφ).exactly_approximates π)
+  {N : near_litter} {B : extended_index β} (hN : ((φ B).litter_map N.1).dom)
+  (hπL : struct_perm.derivative B π • N.1 = (((φ B).litter_map N.1).get hN).1) :
+  ((struct_perm.derivative B π • N : near_litter) : set atom) =
+  ((φ B).litter_map N.1).get hN ∆ (struct_perm.derivative B π • (litter_set N.1 ∆ N)) :=
+begin
+  have := (φ B).smul_near_litter_eq_of_precise_at (hπ B) hN (hφp B hN) _,
+  { rw struct_perm.of_bot_smul at this,
+    exact this, },
+  { rw struct_perm.of_bot_smul,
+    exact hπL, },
+end
+
+end precise
+
+variables {α : Λ} [position_data.{}] [phase_2_assumptions α] {β : Iio α}
+
+/-- A structural action *supports* a tangle if it defines an image for everything
+in the reduction of its designated support. -/
+structure supports (φ : struct_action β) (t : tangle β) : Prop :=
+(atom_mem : ∀ a B, (inl a, B) ∈ reduction α (designated_support t : set (support_condition β)) →
+  ((φ B).atom_map a).dom)
+(litter_mem : ∀ (L : litter) B,
+  (inr L.to_near_litter, B) ∈ reduction α (designated_support t : set (support_condition β)) →
+  ((φ B).litter_map L).dom)
+
+/-- Two structural actions are *compatible* for a tangle if they both support the
+tangle and agree on the reduction of its designated support. -/
+structure compatible (φ ψ : struct_action β) (t : tangle β) : Prop :=
+(φ_supports : φ.supports t)
+(ψ_supports : ψ.supports t)
+(atom_map : ∀ a B ha, ((φ B).atom_map a).get (φ_supports.atom_mem a B ha) =
+  ((ψ B).atom_map a).get (ψ_supports.atom_mem a B ha))
+(litter_map : ∀ L B hL, ((φ B).litter_map L).get (φ_supports.litter_mem L B hL) =
+  ((ψ B).litter_map L).get (ψ_supports.litter_mem L B hL))
+
+/-- The action of a structural action on support conditions. -/
+noncomputable def support_condition_map_or_else (φ : struct_action β) :
+  support_condition β → support_condition β
+| (inl a, B) := (inl ((φ B).atom_map_or_else a), B)
+| (inr N, B) := (inr ((φ B).near_litter_map_or_else N), B)
+
+def coherent_coe (φ : struct_action β) (hφ : φ.lawful) (t : tangle β) : Prop :=
+∀ {π : allowable β} (hπ : (φ.complete hφ).exactly_approximates π.to_struct_perm)
+  (γ : Iic α) (δ ε : Iio α) (hδ : (δ : Λ) < γ) (hε : (ε : Λ) < γ) (hδε : δ ≠ ε)
+  (C : path (β : type_index) γ) (t' : tangle δ) (hL)
+  (hc₁ : ∃ (d : support_condition β), d ∈ (designated_support t).carrier ∧
+    relation.refl_trans_gen (constrains α β)
+    (inr (f_map (coe_ne_coe.mpr (coe_ne' hδε)) t').to_near_litter,
+      (C.cons (coe_lt hε)).cons (bot_lt_coe _)) d)
+  (hc₂ : ∀ (c : support_condition δ), c ∈ (designated_support t').carrier →
+    π • (show support_condition β, from (c.fst, (C.cons (coe_lt hδ)).comp c.snd)) =
+      φ.support_condition_map_or_else (c.fst, (C.cons (coe_lt hδ)).comp c.snd)),
+  f_map (subtype.coe_injective.ne (Iio.coe_injective.ne hδε))
+      (show tangle δ, from
+        (show allowable δ, from allowable_derivative (γ : Iic_index α) δ (coe_lt_coe.mpr hδ)
+          (allowable.derivative
+            (show path ((β : Iic_index α) : type_index) (γ : Iic_index α), from C) π)) • t') =
+    (((φ ((C.cons (coe_lt hε)).cons (bot_lt_coe _))).litter_map
+      (f_map (subtype.coe_injective.ne (Iio.coe_injective.ne hδε)) t')).get hL).fst
+
+def coherent_bot (φ : struct_action β) (hφ : φ.lawful) : Prop :=
+∀ {π : allowable β} (hπ : (φ.complete hφ).exactly_approximates π.to_struct_perm)
+  (γ : Iic α) (ε : Iio α) (hε : (ε : Λ) < γ)
+  (C : path (β : type_index) γ) (a : tangle ⊥) (hL)
+  (hc : struct_perm.derivative (C.cons (bot_lt_coe _)) π.to_struct_perm • a =
+    (φ (C.cons (bot_lt_coe _))).atom_map_or_else a),
+  f_map (show ((⊥ : Iio_index α) : type_index) ≠ (ε : Iio_index α),
+    from subtype.coe_injective.ne Iio_index.bot_ne_coe)
+      ((show allowable (⊥ : Iio_index α), from
+        (allowable.derivative (show path ((β : Iic_index α) : type_index) (⊥ : Iic_index α), from
+          C.cons (bot_lt_coe _))) π) • a) =
+    (((φ ((C.cons (coe_lt hε)).cons (bot_lt_coe _))).litter_map
+      (f_map (show (⊥ : type_index) ≠ (ε : Λ), from bot_ne_coe) a)).get hL).fst
+
+@[mk_iff] structure coherent (φ : struct_action β) (hφ : φ.lawful) (t : tangle β) : Prop :=
+(coe : φ.coherent_coe hφ t)
+(bot : φ.coherent_bot hφ)
+
+lemma smul_litter_eq_of_supports (φ : struct_action β) (hφ : φ.lawful)
+  {π : allowable β} (hπ : (φ.complete hφ).exactly_approximates π.to_struct_perm)
+  (t : tangle β) (hφc : φ.coherent hφ t) (hφs : φ.supports t)
+  (d : support_condition β) (hd : d ∈ designated_support t)
+  (B : extended_index β) (L : litter)
+  (ih : ∀ (e : support_condition β),
+    relation.trans_gen (constrains α β) e (inr L.to_near_litter, B) →
+    π • e = φ.support_condition_map_or_else e)
+  (hc : relation.refl_trans_gen (constrains α β) (inr L.to_near_litter, B) d) :
+  struct_perm.derivative B π.to_struct_perm • L =
+  (((φ B).litter_map L).get
+    (hφs.litter_mem L B ⟨⟨d, hd, refl_trans_gen_near_litter hc⟩, reduced.mk_litter _ _⟩)).fst :=
+begin
+  by_cases hflex : inflexible α L B,
+  { rw inflexible_iff at hflex,
+    obtain (⟨γ, δ, ε, hδ, hε, hδε, C, t', rfl, rfl⟩ | ⟨γ, ε, hε, C, a, rfl, rfl⟩) := hflex,
+    { have hc₂ := λ c hc, ih _ (relation.trans_gen.single $ constrains.f_map hδ hε hδε C t' c hc),
+      have := smul_f_map (δ : Iio_index α) ε _ _ (Iio.coe_injective.ne hδε)
+        (allowable.derivative
+          (show path ((β : Iic_index α) : type_index) (γ : Iic_index α), from C) π) t',
+      rw [← allowable.derivative_cons_apply, allowable.derivative_smul,
+        ← struct_perm.derivative_bot_smul, ← struct_perm.derivative_cons] at this,
+      exact this.trans (hφc.coe hπ γ δ ε hδ hε hδε C t' _ ⟨d, hd, hc⟩ hc₂), },
+    { have hc : (_, _) = (_, _) := ih _ (relation.trans_gen.single $ constrains.f_map_bot hε C a),
+      simp only [smul_inl, prod.mk.inj_iff, eq_self_iff_true, and_true] at hc,
+      rw ← hφc.bot hπ γ ε hε C a _ hc,
+      have := smul_f_map (⊥ : Iio_index α) ε _ _ (by intro h; cases h)
+        (allowable.derivative
+          (show path ((β : Iic_index α) : type_index) (γ : Iic_index α), from C) π) a,
+      rw [← allowable.derivative_cons_apply, allowable.derivative_smul,
+        ← struct_perm.derivative_bot_smul, ← struct_perm.derivative_cons,
+        ← allowable.derivative_cons_apply] at this,
+      exact this, }, },
+  { have := hφs.litter_mem L B ⟨⟨d, hd, refl_trans_gen_near_litter hc⟩, reduced.mk_litter _ _⟩,
+    rw [← struct_perm.of_bot_smul, ← (hπ B).map_litter _ (or.inl (or.inl ⟨this, hflex⟩))],
+    refine ((φ B).complete_smul_litter_eq L).trans _,
+    rw [near_litter_action.flexible_litter_perm_apply_eq, (φ B).rough_litter_map_or_else_of_dom],
+    exact this,
+    exact hflex, },
+end
+
+lemma smul_support_condition_eq (φ : struct_action β) (hφ : φ.lawful) (hφp : φ.precise)
+  {π : allowable β} (hπ : (φ.complete hφ).exactly_approximates π.to_struct_perm)
+  (t : tangle β) (hwc : φ.coherent hφ t) (hws : φ.supports t)
+  (c d : support_condition β)
+  (hc : relation.refl_trans_gen (constrains α β) c d)
+  (hd : d ∈ designated_support t) :
+  π • c = φ.support_condition_map_or_else c :=
+begin
+  revert d,
+  refine (constrains_wf α β).trans_gen.induction c _,
+  rintros c ih d hc hd,
+  obtain ⟨a | N, B⟩ := c,
+  { refine prod.ext _ rfl,
+    change inl _ = inl _,
+    refine congr_arg inl _,
+    rw [φ.smul_atom_eq hπ (hws.atom_mem a B ⟨⟨d, hd, hc⟩, reduced.mk_atom a B⟩),
+      near_litter_action.atom_map_or_else_of_dom], },
+  refine prod.ext _ rfl,
+  change inr _ = inr _,
+  refine congr_arg inr (set_like.coe_injective _),
+  have ih' := λ e he, ih e (relation.trans_gen.single he) d
+    (relation.refl_trans_gen.head he hc) hd,
+  rw φ.smul_near_litter_eq_of_precise hφp hπ (hws.litter_mem N.1 B _) _,
+  { simp only [near_litter_action.near_litter_map_or_else,
+      near_litter.coe_mk, subtype.coe_mk],
+    rw (φ B).litter_map_or_else_of_dom (hws.litter_mem N.1 B _),
+    congr' 1,
+    ext a : 1,
+    rw [mem_smul_set, mem_image],
+    split,
+    { rintro ⟨b, hb₁, hb₂⟩,
+      have : (_, _) = (_, _) := ih' _ (constrains.symm_diff N _ hb₁ B),
+      simp only [smul_inl, smul_inv_smul, prod.mk.inj_iff] at this,
+      rw this.1 at hb₂,
+      exact ⟨b, hb₁, hb₂⟩, },
+    { rintro ⟨b, hb₁, hb₂⟩,
+      have : (_, _) = (_, _) := ih' _ (constrains.symm_diff N _ hb₁ B),
+      simp only [smul_inl, smul_inv_smul, prod.mk.inj_iff] at this,
+      rw ← this.1 at hb₂,
+      exact ⟨b, hb₁, hb₂⟩, },
+    { exact ⟨⟨d, hd, refl_trans_gen_near_litter hc⟩, reduced.mk_litter _ _⟩, }, },
+  refine φ.smul_litter_eq_of_supports hφ hπ t hwc hws d hd B N.1 _ (refl_trans_gen_near_litter hc),
+  exact λ e he, ih e (trans_gen_near_litter he) d
+    (relation.refl_trans_gen.trans he.to_refl (refl_trans_gen_near_litter hc)) hd,
+end
+
+lemma smul_eq_smul_tangle (φ ψ : struct_action β)
+  (hφ : φ.lawful) (hψ : ψ.lawful)
+  (hφp : φ.precise) (hψp : ψ.precise)
+  (t : tangle β) (h : compatible φ ψ t)
+  (hφc : φ.coherent hφ t) (hψc : ψ.coherent hψ t)
+  {πφ πψ : allowable β}
+  (hπφ : (φ.complete hφ).exactly_approximates πφ.to_struct_perm)
+  (hπψ : (ψ.complete hψ).exactly_approximates πψ.to_struct_perm) :
+  πφ • t = πψ • t :=
+begin
+  rw [smul_eq_iff_eq_inv_smul, smul_smul],
+  symmetry,
+  refine (designated_support t).supports _ _,
+  intros c hc,
+  rw [mul_smul, inv_smul_eq_iff],
+  symmetry,
+  rw smul_support_condition_eq φ hφ hφp hπφ t hφc h.φ_supports c c relation.refl_trans_gen.refl hc,
+  rw smul_support_condition_eq ψ hψ hψp hπψ t hψc h.ψ_supports c c relation.refl_trans_gen.refl hc,
+  obtain ⟨a | N, B⟩ := c,
+  { simp only [support_condition_map_or_else, prod.mk.inj_iff, eq_self_iff_true, and_true],
+    rw [(φ B).atom_map_or_else_of_dom, (ψ B).atom_map_or_else_of_dom],
+    refine h.atom_map a B _,
+    exact ⟨⟨_, hc, relation.refl_trans_gen.refl⟩, reduced.mk_atom _ _⟩, },
+  { simp only [support_condition_map_or_else, prod.mk.inj_iff, eq_self_iff_true, and_true,
+      near_litter_action.near_litter_map_or_else],
+    refine set_like.coe_injective _,
+    simp only [near_litter.coe_mk, subtype.coe_mk],
+    congr' 1,
+    { rw [(φ B).litter_map_or_else_of_dom, (ψ B).litter_map_or_else_of_dom, h.litter_map N.1 B _],
+      exact ⟨⟨_, hc, refl_trans_gen_near_litter relation.refl_trans_gen.refl⟩,
+        reduced.mk_litter _ _⟩, },
+    { ext a : 1,
+      rw [mem_image, mem_image],
+      split;
+      rintro ⟨b, hb₁, hb₂⟩;
+      refine ⟨b, hb₁, _⟩;
+      rw [← hb₂, (φ B).atom_map_or_else_of_dom, (ψ B).atom_map_or_else_of_dom],
+      { refine (h.atom_map b B _).symm,
+        exact ⟨⟨_, hc, relation.refl_trans_gen.single (constrains.symm_diff N b hb₁ B)⟩,
+          reduced.mk_atom _ _⟩, },
+      { refine h.atom_map b B _,
+        exact ⟨⟨_, hc, relation.refl_trans_gen.single (constrains.symm_diff N b hb₁ B)⟩,
+          reduced.mk_atom _ _⟩, }, }, },
+end
+
+end struct_action
+
+end con_nf
